\documentclass{ximera}

\input{../preamble}

\outcome{Integrate a Power Series}

\title{3.13 Integrating Power Series}

\begin{document}

\begin{abstract}
We integrate power series term by term.
\end{abstract}

\maketitle

\section{Integration of Power Series}


Suppose that the power series 
\[
\sum_{n=0}^\infty a_n x^n
\]
converges for all $x$ in some open interval $I$. Then, on this interval, the power series has an anti-derivative which can be obtained by integrating term-by-term:


\[
\int \left( \sum_{n=0}^\infty a_n x^n \right) \, dx  = \sum_{n=0}^\infty  \int a_n x^n \, dx   
= \sum_{n=0}^\infty   \frac{a_n}{n+1} x^{n+1} + C.
\]
In other words, the indefinite integral of a power series is computed term by term, as we would anti-differentiate a polynomial.

\begin{example}
The power series 
\[
\sum_{n=0}^\infty x^n
\]
converges on the interval $(-1, 1)$.
On that interval, its anti-derivative is given by
\[
\int\left( \sum_{n=0}^\infty x^n \right) \, dx= \sum_{n=0}^\infty  \big(\int x^n \, dx\big) = \sum_{n=0}^\infty \frac{x^{n+1}}{n+1} + C.
\]

\end{example}



\begin{problem}(problem 1)
Find the anti-derivatives of the following power series:
\[
\sum_{n=0}^\infty \frac{x^n}{n+1},\qquad \sum_{n=0}^\infty \frac{x^n}{2^n},
\]
\[
 \sum_{n=0}^\infty \frac{x^n}{n!},\qquad \sum_{n=0}^\infty x^{2n}
\]
\end{problem}


\end{document}


\begin{example} %example #15
Find $h'(x)$ if $h(x) = x^{\sin(x)}$.\\
We will use the fact that the exponential and logarithm functions are inverses,
\[e^{\ln(x)} = x,\]
and the exponent property of logarithms, 
\[\ln(x^n) = n\ln(x),\]
to rewrite $h(x)$.  We have 
\[h(x) = x^{\sin(x)} = e^{\ln(x^{\sin(x)})} = e^{\sin(x)\ln(x)}\]
and we can now compute $h'(x)$ using a combination of the chain rule and product rule.
We can write $h(x)$ as a composition, $f(g(x))$ with 
\[g(x) = \sin(x)\ln(x) \quad \text{and} \quad f(x) = e^x.\]
Then to find $g'(x)$ we us the product rule and we get $g'(x) = \frac{\sin(x)}{x} + \cos(x)\ln(x)$.
Next $f'(x) = e^x$ and 
hence $f'(g(x)) = e^{g(x)} = e^{\sin(x)\ln(x)} = x^{\sin(x)}$.
We can then conclude $h'(x) = f'(g(x))g'(x) = x^{\sin(x)} \left[ \frac{\sin(x)}{x} + \cos(x)\ln(x)\right]$.
\end{example}

%more question formats below













%\begin{verbatim}
\begin{question}
What is your favorite color?
\begin{multipleChoice}
\choice[correct]{Rainbow}
\choice{Blue}
\choice{Green}
\choice{Red}
\end{multipleChoice}
\begin{freeResponse}
Hello
\end{freeResponse}
\end{question}
%\end{verbatim}





\begin{question}
  Which one will you choose?
  \begin{multipleChoice}
    \choice[correct]{I'm correct.}
    \choice{I'm wrong.}
    \choice{I'm wrong too.}
  \end{multipleChoice}
\end{question}


\begin{question}
  Which one will you choose?
  \begin{selectAll}
    \choice[correct]{I'm correct.}
    \choice{I'm wrong.}
    \choice[correct]{I'm also correct.}
    \choice{I'm wrong too.}
  \end{selectAll}
\end{question}


\begin{freeResponse}
What is the chain rule used for?
\end{freeResponse}
