\documentclass[handout]{ximera}

\input{../preamble}

\pgfplotsset{compat=1.13}

\outcome{Derive the Cauchy-Riemann Equations}

\title{3.3 Cauchy-Riemann Equations}

\begin{document}

\begin{abstract}
We derive the Cauchy-Riemann equations.
\end{abstract}

\maketitle

Recall the definition of partial derivative from multi-variable calculus.  
Let $u(x,y)$ be defined in a neighborhood of $(x_0,y_0)$, then its partial derivatives are defined by

\[
u_x(x_0, y_0) = \frac{\partial u}{\partial x}\Bigg|_{(x_0,y_0)} = \lim_{h \to 0} \frac{u(x_0 +h, y_0) - u(x_0,y_0)}{h}
\]

and

\[
u_y(x_0, y_0) = \frac{\partial u}{\partial y}\Bigg|_{(x_0,y_0)} = \lim_{h \to 0} \frac{u(x_0 , y_0+h) - u(x_0,y_0)}{h}
\]

In the definition of $f'(z_0)$ we can let $h$ approach $0$ along any path. If we choose $h$ to be real, then we get a powerful result.
\begin{theorem}
If $f(z) = u(x,y) + iv(x,y)$ is differentiable at $z_0 = x_0 + iy_0$, then
\[
f'(z_0) = u_x(x_0,y_0) + iv_x(x_0,y_0)
\]
\end{theorem}

\begin{remark}
In short, we can write
\[
f' = f_x = u_x + iv_x
\]
\end{remark}

\begin{proof}
We let $h$ approach $0$ along the $x$-axis in the definition of $f'(z_0)$:
\begin{align*}
f'(z_0) &= \lim_{h \to 0 \atop h \in \R} \frac{f(z_0 + h) -f(z_0)}{h} \\[10pt]
        &= \lim_{h \to 0} \frac{\left[u(x_0 +h, y_0) + iv(x_0 +h, y_0)\right] - \left[u(x_0,y_0)+iv(x_0, y_0)\right]}{h} \\[10pt]
        &=  \lim_{h \to 0} \frac{u(x_0 +h, y_0)- u(x_0,y_0)}{h} +i\lim_{h \to 0}\frac{v(x_0 +h, y_0)-v(x_0, y_0)}{h} \\[10pt]
        &= u_x(x_0,y_0) + iv_x(x_0,y_0)
\end{align*}
\end{proof}




\begin{example}
Find $f'(z)$ for the complex exponential function $f(z) = e^z$.\\
Since $e^z = e^x \cos y + i e^x \sin y$, we have
\[
u_x = u_x(x,y) = \frac{\partial}{\partial x} \left(e^x \cos y \right)= e^x \cos y 
\]
and
\[
 v_x = v_x(x,y) = \frac{\partial}{\partial x}\left(e^x \sin y\right) = e^x \sin y
\]
Thus, 
\[
f'(z_0) = e^{x_0} \cos y_0 + i e^{x_0} \sin y_0  = e^{z_0}
\]
for any $z_0 = x_0 + iy_0 \in \C$.
Thus, we can write
\[
\frac{d}{dz} e^z = e^z \;\; \mbox{for all} \;\; z \in \C
\]
\end{example}


\begin{problem}
Show that
\[
\frac{d}{dz} \sin z = \cos z \quad \mbox{and} \quad \frac{d}{dz} \cos z = -\sin z
\]
for all $z \in \C$.
\begin{hint}
$\sin z = \sin x \cosh y + i \cos x \sinh y$
\end{hint}
\begin{hint}
$\cos z = \cos x \cosh y - i \sin x \sinh y$
\end{hint}
\end{problem}

In the theorem above, we computed $f'(z_0)$ by letting $h$ be real.  Suppose we let $h$ be purely imaginary, instead.
Let $h = ik$ where $k \in \R$, then
\begin{align*}
f'(z_0) &= \lim_{h \to 0 \atop h = ik} \frac{f(z_0 + h) -f(z_0)}{h} \\[10pt]
        &= \lim_{k \to 0 \atop k \in \R} \frac{\left[u(x_0 , y_0+k) + iv(x_0 , y_0+k)\right] - \left[u(x_0,y_0)+iv(x_0, y_0)\right]}{ik} \\[10pt]
        &=  \lim_{k \to 0} \frac{u(x_0 , y_0+k)- u(x_0,y_0)}{ik} +i\lim_{k \to 0}\frac{v(x_0 , y_0+k)-v(x_0, y_0)}{ik} \\[10pt]
        &= -iu_y(x_0,y_0) + v_y(x_0,y_0)\\
        &=  v_y(x_0,y_0)-iu_y(x_0,y_0)
\end{align*}

Thus we see that we could have written $f'$ as
\[
f'(z_0) = v_y(x_0,y_0)-iu_y(x_0,y_0)
\]

Now, we have two different forms for $f'(z_0)$ which depend on the direction in which $h$ approached $0$.
By assumption, $f$ was differentiable at $z_0$, so these two forms must be equal. This gives rise to the Cauchy-Riemann Equations.
\begin{theorem}[Cauchy-Riemann Equations]
Suppose $f(z)$ is differentiable at $z = z_0 = x_0 +iy_0$. Then
\[
v_x(x_0,y_0)= -u_y(x_0,y_0) 
\]
and 
\[
v_y(x_0,y_0) = u_x(x_0,y_0)
\]
In short, 
\[
u_x =v_y \quad \mbox{and} \quad u_y = -v_x
\]
\end{theorem}
\begin{proof}
Since $f$ is differentiable at $z_0$, we can let $h$ be either purely real or purely imaginary in the definition of $f'(z_0)$
and the results must be equal. Therefore
\[
f'(z_0) = u_x(x_0,y_0)+iv_x(x_0,y_0)
\]
and
\[
f'(z_0) = v_y(x_0,y_0)-iu_y(x_0,y_0)
\]
The result follows by equating the real and imaginary parts.
\end{proof}
\begin{remark}
The Cauchy-Riemann Equations can be written in a single complex equation instead of two real equations as
\[
f_y = if_x
\]
\end{remark}

Some functions, like $\Log z$ and $z^{1/2}$, are best described using polar coordinates. To determine their derivatives, we need 
to express $f'(z)$ in terms of $u_r, u_\theta, v_r$ and $v_\theta$. To do this, we will take advantage of the polar coordinate transformations,
\[
x = r\cos \theta \quad \mbox{and} \quad y=r\sin \theta
\]
and the multivariate version of the chain rule.
Suppose $f(z) = u(x,y) + iv(x,y)$ is differentiable at $z = x+iy$.
Then, by the multivariate chain rule,
\begin{align*}
\frac{\partial u}{\partial r} &= \frac{\partial u}{\partial x}\frac{\partial x}{\partial r}+\frac{\partial u}{\partial y}\frac{\partial y}{\partial r}\\
                              &= \frac{\partial u}{\partial x} \cos\theta + \frac{\partial u}{\partial y} \sin \theta
\end{align*}
In short
\[
u_r = u_x \cos \theta + u_y \sin\theta
\]
\begin{problem}
Show that
\[
u_\theta = -ru_x \sin \theta + ru_y \cos\theta
\]
\end{problem}

Similarly,

\[
 v_r = v_x \cos \theta + v_y \sin\theta \quad \mbox{and} \quad  v_\theta = -rv_x \sin \theta + rv_y \cos\theta
\]

By the Cauchy-Riemann Equations, $u_x = v_y$ and $u_y = -v_x$ we have
%and substituting for $v_x$ and $v_y$ in $v_r$ and $v_\theta$ from the problem above, gives
\[
v_r = -u_y \cos \theta + u_x \sin\theta \quad \mbox{and} \quad  v_\theta = ru_y \sin \theta + ru_x \cos\theta
\]
Now, we can observe the Cauchy-Riemann Equations in polar form:
\[
u_r = \frac{1}{r} v_\theta \quad \mbox{and} \quad u_\theta = -rv_r
\]
Finally, we would like to formulate $f'(z) = u_x + iv_x$, in terms of $u_r$ and $v_r$.
\begin{problem} Solve the $2 \times 2$ system of equations
\begin{align*}
u_r &= u_x \cos \theta + u_y \sin\theta\\
v_r &= u_x \sin \theta -u_y \cos\theta
\end{align*}
for $u_x$ and $u_y$
\begin{multipleChoice}
\choice{$u_x = u_r \cos \theta - v_r \sin \theta$ \quad and \quad $u_y = u_r \sin \theta + v_r \cos \theta $}
\choice{$u_x = u_r \sin \theta + v_r \cos \theta$ \quad and \quad $u_y = u_r \cos \theta - v_r \sin \theta $}
\choice[correct]{$u_x = u_r \cos \theta + v_r \sin \theta$ \quad and \quad $u_y = u_r \sin \theta - v_r \cos \theta $}
\end{multipleChoice}
\end{problem}

From the Cauchy-Riemann Equation, $v_x = -u_y$, and the result of the previous problem, we can write
\begin{align*}
f'(z) &= u_x + iv_x\\
      & = u_x - iu_y\\
      &= \left[u_r \cos \theta + v_r \sin \theta\right] - i\left[ u_r \sin \theta - v_r \cos \theta \right]\\
      &= \left[u_r \cos \theta -i u_r \sin \theta\right] + i\left[ v_r \cos \theta  - iv_r \sin \theta\right]\\
      &= u_r e^{-i\theta} + v_r e^{-i\theta}\\
      &=  e^{-i\theta}(u_r +v_r)
\end{align*}

We have just proved the following theorem:

\begin{theorem}
If $f(z) = f\left(re^{i\theta}\right)$ is differentiable at $z = z_0 = r_0 e^{i\theta_0}$ then
\[
f'(z_0) = e^{-i\theta_0} \left[u_r(r_0, \theta_0) + v_r(r_0, \theta_0)\right]
\]
\end{theorem}

\begin{example}
Use the theorem above to find the derivative of $f(z) = \Log z$ at $z = z_0$ where $z_0$ is in the 
slit plane $\C \backslash \{x\leq 0, y=0\}$ \\
We can write $z_0 = r_0 e^{i\theta_0}$ where $\theta_0 = \Arg z_0$. Since $\Log z = \ln r + i\theta$
where $\theta = \Arg z$, we have 
\[
u_r(r_0,\theta_0) = \frac{1}{r_0} \quad \mbox{and} \quad v_r(r_0,\theta_0) = 0
\]
Hence, according to the theorem,
\begin{align*}
f'(z_0) &= e^{-i\theta_0}[u_r(r_0,\theta_0)+v_r(r_0,\theta_0)] \\
        &= e^{-i\theta_0}\frac{1}{r_0}\\
        &= \frac{1}{e^{i\theta_0}r_0}\\
        &= \frac{1}{z_0}
\end{align*}
Dropping the subscript, we can write
\[
\frac{d}{dz} \Log z = \frac{1}{z}
\]
for $z$ in the slit plane.
\end{example}

\begin{problem} Let $z_0$ be in the slit plane, $\C \backslash \{x\leq 0, y=0\}$. 
Find $f'(z_0)$ if $f(z) = z^{1/2}$, the principal branch of the square root function.
\begin{hint}
$\displaystyle z^{\frac12} = r^{\frac12}e^{i\frac{\theta}{2}}$ where $\theta = \Arg z$
\end{hint}
\end{problem}

\end{document}





