\documentclass{ximera}
%\usepackage{tcolorbox}
\input{../preamble}

\outcome{Learn the Power Rule for differentiating power functions}

\title{2.1 Power Rule}

%\newcommand{\ffrac}[2]{\frac{\mbox{\footnotesize $#1$}}{\mbox{\footnotesize $#2$}}}
%\newcommand{\vasymptote}[2][]{
%    \draw [densely dashed,#1] ({rel axis cs:0,0} -| {axis cs:#2,0}) -- ({rel axis cs:0,1} -| {axis cs:#2,0});
%}


\begin{document}

\begin{abstract}
We learn how to find the derivative of a power function.
\end{abstract}

\maketitle

\youtube{bRZmfc1YFsQ}

\section{The Power Rule}

In this section we present the derivatives power functions. A power function is a function of the form $f(x) = x^\text{n}$.  

\begin{theorem}[Power Rule]
For any number n, the derivative of the power function $f(x) = x^\text{n}$ is given by
$f'(x) = \text{n}x^{\text{n} -1}$, i.e.,
\[\frac{d}{dx} \left(x^\text{n}\right) = \text{n}x^{\text{n}-1}.\]
\end{theorem}

We will investigate this rule in the case where n is a whole number. The key is to use 
the \link[Binomial Theorem]{https://en.wikipedia.org/wiki/Binomial_theorem}, which gives a formula for 
expanding powers of $x+h$. 
Here are some examples of the theorem:

\begin{eqnarray*}
(x+h)^{\bf 2} &=&x^2 + {\bf 2}xh + h^2\\
(x+h)^{\bf 3} &=& x^3 + {\bf 3}x^2h + 3xh^2 + h^3\\
(x+h)^{\bf 4} &=& x^4 + {\bf 4}x^3h+ 6x^2h^2 + 4xh^3 + h^4\\
(x+h)^{\bf 5} &=& x^5 + {\bf 5}x^4h + 10x^3h^2 + 10x^2h^3 + 5xh^4 + h^5
\end{eqnarray*}

The coefficients can be  determined using a device called \link[Pascal's Triangle]{https://en.wikipedia.org/wiki/Pascal's_triangle}.
Notice that the coefficient of the second term on the right hand side always matches the power on the left hand side. In general,

\[(x+h)^{\bf \text{n}} = x^\text{n} + {\bf \text{n}}x^{\text{n}-1}h + \dots + \text{n}xh^{\text{n}-1} + h^\text{n}.\]

Also observe that as the powers of $x$ decrease, the powers of $h$ increase.\\

We will now use the definition of the derivative to discover the power rule. 
Let $f(x) = x^\text{n}$, where \text{n} is a whole number. Then

\begin{eqnarray*}
f'(x) &=& \lim_{h\to 0} \frac{f(x+h)-f(x)}{h}\\[10 pt] 
&=& \lim_{h\to 0} \frac{(x+h)^\text{n}-x^\text{n}}{h}\\[10 pt]
&=& \lim_{h\to 0} \frac{\left(x^\text{n} + \text{n}x^{\text{n}-1}h + \dots + \text{n}xh^{\text{n}-1} + h^\text{n}\right)-x^\text{n}}{h}\\[10 pt]
 &=& \lim_{h\to 0} \frac{\text{n}x^{\text{n}-1}h + \dots + \text{n}xh^{\text{n}-1} + h^\text{n}}{h} \\[10 pt]
 &=& \lim_{h\to 0} \left(\text{n}x^{\text{n}-1} + \dots + \text{n}xh^{\text{n}-2} + h^{\text{n}-1}\right) \\[10 pt] 
 &=& \text{n}x^{\text{n}-1}.
 \end{eqnarray*}




\begin{example}[example 1]
Find the derivative of  $f(x) = x^4$.\\
We can use the power rule with $n = 4$ to obtain $f'(x) = 4x^3.$
\end{example}



\begin{problem}(problem 1a)
Compute
\[
\frac{d}{dx} \left(x^3\right).
\]
\begin{hint}
Use the power rule with $n = 3$
\end{hint}
\begin{prompt}
The derivative of $f(x) = x^3$ is \ $f'(x) = \answer{3x^2}.$
\end{prompt}
\end{problem}



\begin{problem}(problem 1b)
Compute
\[
%\frac{d}{dx}
\dd{x} \left(x^5\right).
\]
\begin{hint}
Use the power rule with $n = 5$
\end{hint}
The derivative of $f(x) = x^5$ is \ $f'(x) = \answer{5x^4}.$
\end{problem}



\begin{problem}(problem 1c)
Find the slope of the tangent line to the graph of 
\[
f(x) = x^6  \;\; \text{at} \;\; x = -2.
\]
\begin{hint}
The derivative gives the slope of the tangent line
\end{hint}
\begin{hint}
Use the power rule with $n = 6$
\end{hint}
The slope is  $\answer{-192}.$
\end{problem}


\begin{example}[example 2]
Find the derivative of $f(x) = x^{100}$.\\
We can use the power rule with $n = 100$ to obtain $f'(x) = 100x^{99}.$
\end{example}

\begin{problem}(problem 2)
Compute
\[
\frac{d}{dx} \left(x^{250}\right).
\]
\begin{hint}
Use the power rule with $n = 250$
\end{hint}
The derivative of $x^{250}$ is $\answer{250x^{249}}.$
\end{problem}



\begin{example}[example 3]
Find the derivative of $f(x) = 1$.\\
We can rewrite the function as a power function, since $x^0 = 1$ and then we can use the power rule with $n=0$. We get $f'(x) = 0x^{-1} = 0$. 
We can also arrive at this answer using a gemoetric understanding of the derivative.
The graph of the constant function $f(x) = 1$ is a horizonatal line which has slope 0. 
Since the derivative is the slope of the tangent line, the derivative is 0.
For this reason, the derivative of any constant function is 0, as stated in the following propsition.
\end{example}

\begin{proposition}[Constant Functions]
If $c$ is any constant, then
\[
\frac{d}{dx} \left(c\right) = 0.
\]
\end{proposition}

The graph of a constant function is a horizontal line with slope 0.
The graphs of $y = -2$, $y = 1/2$ and $y = 3$ are shown below.
(To see $y=3$, zoom out by clicking on the minus in the graphing window or 
by placing the cursor in the graphing window and using the scroll wheel on your mouse).
\[
\graph{y = 3, y = 1/2, y = -2}
\]



\begin{example}[example 4]
If $f(x) = 5, -7, \frac23$ or $4.15$, then $f'(x) = 0$ 
because these are all constants. Notice that none of the expressions contain the variable $x$.
\end{example}



\begin{example}[example 5]
If $f(x) = -\pi, e^3, \sqrt 2$ or $\ln(8)$, then $f'(x) = 0$ 
because these are all constants. Notice that none of the expressions contain the variable $x$.
\end{example}



\begin{problem}(problem 5)
Compute
\[
\frac{d}{dx} \left(94.1\right) = \answer{0}
\]

\[
\frac{d}{dx} \left(\pi^2\right) = \answer{0}
\]

\[
\frac{d}{dt} \left( \sqrt 5 \right) = \answer{0}
\]


\end{problem}



\begin{example}[example 6]
Find the derivative of $f(x) = x$.\\
We can use the power rule with $n=1$ to obtain $f'(x) = 1x^0 = 1$. 
This answer can also be arrived at by interpreting the derivative as slope. The graph of the function $f(x) = x$ is a straight line with slope $1$,
so the derivative is $1$.  More generally, the graph of a function $f(x) = mx$
is a line with slope $m$, so the derivative of $mx$ is $m$.
\end{example}

\begin{problem}(problem 6)
\[
\frac{d}{dt}\left(t\right) = \answer{1}
\]
\end{problem}


\begin{proposition}[Linear Functions]
For any number $m$,
\[
\frac{d}{dx} (mx) = m.
\]
\end{proposition}


The graph of $f(x) = mx$ is a line with slope $m$.
The graphs of $y = 2x$, $y = x/2$ and $y = -x$ are shown below.
Which one is which? Click on the double arrows in the upper left hand corner of the graphing window to check your answer.
\[
\graph{2x, x/2, -x}
\]



\begin{example}[example 7]
If $f(x) = -3x$ then $f'(x) = -3$.
\end{example}



\begin{problem}(problem 7a)
If $f(x) = 4x$ then $f'(x) = \answer{4}$
\end{problem}

\begin{problem}(problem 7b)
If $g(t) = -2t$ then $g'(t) = \answer{-2}$
\end{problem}



\begin{example}[example 8]
If $f(x) = \pi x$ then $f'(x) = \pi$.
\end{example}

\begin{problem}(problem 8a)
\[
\frac{d}{dx} \left(ex\right) = \answer{e}
\]
\end{problem}



\begin{problem}(problem 8b)
\[
\frac{d}{dx} \left(x\ln(5)\right) = \answer{\ln(5)}
\]
\end{problem}






\begin{example}[example 9]
If $f(x) = \frac{x}{2}$ then $f'(x) = \frac 12$.
\end{example}



\begin{problem}(problem 9a)
\[
\frac{d}{dx} \left(\frac{x}{3}\right) = \answer{1/3}
\]
\end{problem}



\begin{problem}(problem 9b)
\[
\frac{d}{dx} \left(-\frac{2x}{5}\right) = \answer{-2/5}
\]
\end{problem}






We now consider examples where the exponment $n$ is a fraction. Recall the defintion of rational exponents:
\[
x^{\frac{m}{n}} = \sqrt[n]{x^m}.
\]



\begin{example}[example 10]
Find the derivative of $f(x) = \sqrt x$.\\
We can rewrite $\sqrt x$ as $x^{1/2}$ and use the power rule 
with $n = 1/2$ to obtain $f'(x) = (1/2)x^{-1/2}$.  This can then be rewritten in radical form :
\[(1/2)x^{-1/2} = \frac{1}{2}\cdot \frac{1}{x^{1/2}} = \frac{1}{2\sqrt x}.\]
This result is used frequently, so it is best to remember it as
\[\frac{d}{dx}\left(\sqrt x\right) = \frac{1}{2\sqrt x}.\]
\end{example}




\begin{example}[example 11]
Find the derivative of $f(x) = \sqrt[3] x$.\\
We can rewrite $\sqrt[3] x$ as $x^{1/3}$ and use the power rule with $n = 1/3$ to obtain
$f'(x) = (1/3)x^{-2/3}$.  This can be rewritten in radical form as 
\[(1/3)x^{-2/3} = \frac{1}{3}\cdot \frac{1}{x^{2/3}} = \frac{1}{3\sqrt[3] {x^2}}.\]
\end{example}




\begin{problem}(problem 11a)
Compute
\[
\frac{d}{dx} \left(\sqrt[4] x\right).
\]
\begin{hint}
Rewrite $\sqrt[4] x$ as $x^{1/4}$
\end{hint}
\begin{hint}
Use the power rule with $n = 1/4$
\end{hint}
The derivative of $\sqrt[4] x$ is $\answer{1/4 x^{-3/4}}.$
\end{problem}



\begin{problem}(problem 11b)
Find the slope of the tangent line to the graph of 
\[
f(x) = \sqrt[5] x  \;\; \text{at} \;\; x = -32.
\]

\begin{hint}
The derivative gives the slope of the tangent line
\end{hint}
\begin{hint}
Rewrite $\sqrt[5] x$ as $x^{1/5}$
\end{hint}
\begin{hint}
Use the power rule with $n = 1/5$
\end{hint}
The slope is  $\answer{1/80}.$
\end{problem}



\begin{example}[example 12]
Find the derivative of $f(x) = x^2\sqrt[4] {x^3}$.\\
We first rewrite $f(x)$ 
as $x^2 \cdot x^{3/4} = x^{11/4}$ (adding exponents) and then we use the power rule with $n = 11/4$
to obtain $f'(x) = (11/4)x^{7/4}$. This can be rewritten in radical form as 
\[(11/4)x^{7/4}  = \frac{11}{4} \sqrt[4] {x^7} = \frac{11}{4} x\sqrt[4] {x^3} .\]
\end{example}



\begin{problem}(problem 12)
Compute
\[
\frac{d}{dx} \left(x\sqrt[3] x\right).
\]
\begin{hint}
Rewrite $x\sqrt[3] x$ as $x^{4/3}$
\end{hint}
\begin{hint}
Use the power rule with $n = 4/3$
\end{hint}
The derivative of $x\sqrt[3] x$ is $\answer{(4/3) x^{1/3}}.$
\end{problem}



Next, we look at some examples involving negative exponents. Recall the definition of negative exponents:
\[
x^{-n} = \frac{1}{x^n}.
\]



\begin{example}[example 13]
Find the derivative of $f(x) = \dfrac{1}{x}$.\\
We can rewrite $1/x$ as $x^{-1}$ and use the power rule with $n = -1$ to obtain 
We get $f'(x) = -1x^{-2}$.
This can be rewritten without the negative exponent as
\[ 
-1x^{-2} = -\frac{1}{x^2}.
\]
%This result is used frequently, so it is best to remember it as
%\[
%\frac{d}{dx}\left(\frac{1}{x}\right) = -\frac{1}{x^2}.
%\]
\end{example}



\begin{example}[example 14]
Find the derivative of $f(x) = 1/x^3$.\\
We can rewrite $1/x^3$ as $x^{-3}$ and use the power rule with $n = -3$ to obtain 
$f'(x) = -3x^{-4}$.
This can be rewritten without the negative exponent as
\[
-3x^{-4} = -\frac{3}{x^4}.
\]
\end{example}




\begin{problem}(problem 14a)
Compute
\[
\frac{d}{dx} \left(\frac{1}{x^2}\right).
\]
\begin{hint}
Rewrite $\dfrac{1}{x^2}$ as $x^{-2}$
\end{hint}
\begin{hint}
Use the power rule with $n = -2$
\end{hint}
The derivative of $f(x) = \dfrac{1}{x^2}$ is \ $f'(x) = \answer{-2x^{-3}}.$
\end{problem}




\begin{problem}(problem 14b)
Find the slope of the tangent line to the graph of 
\[
f(x) = \frac{1}{x^3} \;\; \text{at} \;\; x = 3.
\]


\begin{hint}
The derivative gives the slope of the tangent line
\end{hint}
\begin{hint}
Rewrite $\dfrac{1}{x^3}$ as $x^{-3}$
\end{hint}
\begin{hint}
Use the power rule with $n = -3$
\end{hint}
The slope is  $\answer{-1/27}.$
\end{problem}




\begin{example}[example 15]
Find the derivative of $f(x) = \dfrac{1}{\sqrt x}$.\\
We can rewrite $\frac{1}{\sqrt x}$ as $x^{-1/2}$ and use the power rule with $n = -1/2$ to obtain
\[
f'(x) = -\frac12 x^{-3/2}.
\]
This can be rewritten without the negative exponent as
\[
(-1/2)x^{-3/2}= -\frac{1}{2} \cdot \frac{1}{x^{3/2}} = -\frac{1}{2\sqrt{x^3}} = -\frac{1}{2x\sqrt x}.
\]
\end{example}




\begin{problem}(problem 15)
Compute
\[
\frac{d}{dx} \left(\frac{1}{\sqrt[5] x}\right).
\]
\begin{hint}
Rewrite $1/\sqrt[5] x$ as $x^{-1/5}$
\end{hint}
\begin{hint}
Use the power rule with $n = -1/5$
\end{hint}
The derivative of $f(x) = \frac{1}{\sqrt[5] x}$ is \ $f'(x) = \answer{(-1/5) x^{-6/5}}.$
\end{problem}




\begin{example}[example 16]
Find the derivative of $f(x) = \dfrac{\sqrt[3] {x^2}}{\sqrt[4] x}.$\\
We can rewrite $f(x)$ as $\frac{x^{2/3}}{x^{1/4}} = x^{5/12}$ 
(subtracting exponents). Now, we use the power rule with $n = \frac{5}{12}$ to obtain $f'(x) = \tfrac{5}{12}x^{-7/12}.$
This can be rewritten without the negative exponent as
\[
\tfrac{5}{12}x^{-7/12} = \tfrac{5}{12} \cdot \frac{1}{x^{7/12}} = \frac{5}{12\sqrt[12]{x^7}}.
\]
\end{example}




\begin{problem}(problem 16)
Compute
\[
\frac{d}{dx} \left(\frac{\sqrt[4] {x^3}}{\sqrt[3] x}\right).
\]
\begin{hint}
Rewrite $\frac{\sqrt[4] {x^3}}{\sqrt[3] x}$ as $\frac{x^{3/4}}{x^{1/3}} = x^{5/12}$
\end{hint}
\begin{hint}
Use the power rule with $n = 5/12$
\end{hint}
The derivative of $\frac{\sqrt[4] {x^3}}{\sqrt[3] x}$ is $\answer{(5/12) x^{-7/12}}.$
\end{problem}




\begin{center}
\begin{foldable}
\unfoldable{Below is a graph of $f(x) = x^2$ (in blue) and its derivative, $f'(x) = 2x$ (in purple).
Notice that the slope of the tangent line to $f(x)$ (in red) is the height of the corresponding point 
on $f'(x)$.}
\includeinteractive{fd01.js}
%\graph{x^2}
\end{foldable}
\end{center}



\begin{center}
\begin{foldable}
\unfoldable{Below is a graph of $f(x) = x^3$ (in blue) and its derivative, $f'(x) = 3x^2$ (in purple).
Notice that the slope of the tangent line to $f(x)$ (in red) is the height of the corresponding point on $f'(x)$.}
\includeinteractive{fd02.js}
\end{foldable}
\end{center}


%change these functions to x^2 - 3 and a cubic polynomial with 2 turning points, like  x^3 - 12x whose deriv is 3x^2 -12
%this way the horiz tan lines don't go thru the origin


\begin{center}
\begin{foldable}
\unfoldable{Below is a graph of $f(x) = \sqrt[3] x$ (in blue) and its derivative, 
$f'(x) = \frac{1}{3\sqrt[3]x^2}$ (in purple).
Notice that the slope of the tangent line to $f(x)$ (in red) is the height of the corresponding 
point on $f'(x)$.}
\includeinteractive{fd03.js}
\end{foldable}
\end{center}




\end{document}



\begin{example} %example 17
If $f(x) = 2^x$ then $f'(x) = 2^x \ln(2)$.
\end{example}


\begin{example} %example 18
If $f(x) = 10^x$ then $f'(x) = 10^x \ln(10)$.
\end{example}

\begin{problem}
Compute
\[
\frac{d}{dx} 5^x.
\]
\begin{hint}
Use the exponential rule with $a = 5$
\end{hint}
\begin{hint}
The derivative of $a^x$ is $a^x\ln(a)$
\end{hint}
The derivative of $5^x$ is $\answer{5^x\ln(5)}$.
\end{problem}


\begin{example} %example 19
If $f(x) = \log_2(x)$ then $f'(x) = \frac{1}{x\ln(2)}$.
\end{example}


\begin{example} %example 20
If $f(x) = \log(x)$ then $f'(x) = \frac{1}{x\ln(10)}$.
\end{example}








\begin{center}
\begin{foldable}
\unfoldable{Below is a graph of $f(x) = \cos(x)$ (in green) and its derivative, $f'(x) = -\sin(x)$ (in purple).
Notice that the slope of the tangent line to $f(x)$ (in orange) is the height of the corresponding 
point on $f'(x)$.}
\includeinteractive{fd04.js}
\end{foldable}
\end{center}


\begin{center}
\begin{foldable}
\unfoldable{Below is a graph of $f(x) = \tan^{-1}(x)$ (in green) and its derivative, 
$f'(x) = \frac{1}{1+x^2}$ (in purple).
Notice that the slope of the tangent line to $f(x)$ (in orange) is the height of the corresponding 
point on $f'(x)$.}
\includeinteractive{fd05.js}
\end{foldable}
\end{center}






\section{Leibniz Notation}

In this section we introduce another notation for the derivative. The slope of a line segment is given by
\[m = \frac{\text{rise}}{\text{run}} = \frac{\Delta y}{\Delta x}\]
and since the derivative represents a formula for the slope of a tangent line to a curve $y = f(x)$,
a natural notation for the derivative is Leibniz' notation:
\[ f'(x) = \frac{dy}{dx},\]
which closely resembles the delta notation for slope.





\begin{center}

\bf{Examples of Leibniz Notation}

\end{center}


\begin{example} %example 21
If $y = x^2$ then $\displaystyle{\frac{dy}{dx} = 2x.}$
\end{example}

\begin{example} %example 22
If $y = \sqrt x$ then $\displaystyle{\frac{dy}{dx} = \frac{1}{2\sqrt x}.}$
\end{example}

\begin{example} %example 23
If $y = \frac{1}{x}$ then $\displaystyle{\frac{dy}{dx} = -\frac{1}{x^2}.}$
\end{example}

\begin{example} %example 24
If $y = \sin(x)$ then $\displaystyle{\frac{dy}{dx} = \cos(x).}$
\end{example}

\begin{example} %example 25
If $y = \cos(x)$ then $\displaystyle{\frac{dy}{dx} = -\sin(x).}$
\end{example}

There is also a way to describe the derivative using Leibniz style notation without explicitly stating the function first:

\[f'(x) = \frac{d}{dx}[f(x)].\]

Some examples in this format:

\begin{example} %example 26
$\displaystyle{\frac{d}{dx}\big( \tan(x) \big) = \frac{d}{dx} \tan(x) = \sec^2(x).}$
\end{example}

\begin{example} %example 27
$\displaystyle{\frac{d}{dx}\big( \sec(x) \big) = \frac{d}{dx} \sec(x) =\sec(x)\tan(x).}$
\end{example}

\begin{example} %example 28
$\displaystyle{\frac{d}{dx}\big( e^x \big) = e^x.}$
\end{example}

\begin{example} %example 29
$\displaystyle{\frac{d}{dx}\big( \ln(x) \big) = \frac{d}{dx} \ln(x)= \frac{1}{x}.}$
\end{example}

\begin{example} %example 30
$\displaystyle{\frac{d}{dx}\big( \tan^{-1}(x) \big) = \frac{d}{dx} \tan^{-1}(x) = \frac{1}{1+x^2}.}$
\end{example}




















\begin{description}
\item[Constant:] If $f(x) = c$ then $f'(x) = 0$, where $c$ is any constant.
\item[Linear:] If $f(x) = ax$ then $f'(x) = a$, where $a$ is any nonzero constant.
\item[Power Rule:] If $f(x) = x^n$ then $f'(x) = nx^{n-1}$ where $n$ is a nonzero constant.
\item[Trig:] If $f(x) = \sin(x)$ then $f'(x) = \cos(x)$.
\item[Trig:] If $f(x) = \cos(x)$ then $f'(x) = -\sin(x)$.
\item[Trig:] If $f(x) = \tan(x)$ then $f'(x) = \sec^2(x)$.
\item[Trig:] If $f(x) = \sec(x)$ then $f'(x) = \sec(x)\tan(x)$.
\item[Trig:] If $f(x) = \cot(x)$ then $f'(x) = -\csc^2(x)$.
\item[Trig:] If $f(x) = \csc(x)$ then $f'(x) = -\csc(x)\cot(x)$.
\item[Inverse Trig:] If $f(x)  = \sin^{-1}(x)$ then $f'(x) = \frac{1}{\sqrt{1-x^2}}$.
\item[Inverse Trig:] If $f(x)  = \cos^{-1}(x)$ then $f'(x) = -\frac{1}{\sqrt{1-x^2}}$.
\item[Inverse Trig:] If $f(x)  = \tan^{-1}(x)$ then $f'(x) = \frac{1}{1+x^2}$.
\item[Exponential:] If $f(x) = e^x$ then $f'(x) = e^x$.
\item[Exponential:] If $f(x) = a^x$ then $f'(x) = a^x \cdot \ln(a)$.
%where $a>0$ and $a \neq 1$
\item[Log:] If $f(x) = \ln(x)$ then $f'(x) = \frac{1}{x}.$
\item[Log:] If $f(x) = \log_a(x)$ then $f'(x) = \frac{1}{x \ln(a)}.$
\end{description}
