\documentclass{ximera}

\input{../preamble}

\outcome{Differentiate a power series}

\title{3.12 Differentiation of Power Series}

\begin{document}

\begin{abstract}
We differentiate power series term by term.
\end{abstract}

\maketitle



Suppose that the power series 
\[
\sum_{n=0}^\infty a_n x^n
\]
converges for all $x$ in some open interval $I$. Then, on this interval, the power series represents a differentiable function and its derivative is given by 
\[
\frac{d}{dx} \left( \sum_{n=0}^\infty a_n x^n \right) = \sum_{n=0}^\infty  \frac{d}{dx}\big( a_n x^n \big)  
= \sum_{n=1}^\infty   n\cdot a_n x^{n-1}
\]
In other words, the derivative of a power series is a power series. and the derivative is computed term by term, as we would differentiate a polynomial.

\begin{example}[example 1]
Find the derivative of the power series
\[
\sum_{n=0}^\infty x^n
\]
This power series converges on the interval $(-1, 1)$.
On that interval, its derivative is given by
\[
\frac{d}{dx}\left( \sum_{n=0}^\infty x^n \right)= \sum_{n=0}^\infty \frac{d}{dx} \big(x^n\big) = \sum_{n=1}^\infty nx^{n-1}.
\]
We can re-index to rewrite this as
\[
\sum_{n=1}^\infty nx^{n-1} = \sum_{n=0}^\infty (n+1)x^n
\]
We have seen that the original power series above represents the function 
\[
f(x) = \frac{1}{1-x} = \sum_{n=0}^\infty x^n
\]
on the interval $(-1, 1)$. The derivative of this function is
\[
f'(x) = \frac{1}{(1-x)^2} \;\; \text{(verify)}
\]
Thus, we have a power series representation for this function:
\[
\frac{1}{(1-x)^2} = \sum_{n=0}^\infty (n+1)x^n
\]
\end{example}



\begin{problem}(problem 1)
Find the derivatives of the following power series:
\[
a) \; \sum_{n=1}^\infty \frac{x^n}{n},\qquad  b) \; \sum_{n=0}^\infty \frac{x^n}{2^n},
\]
\[
 c) \; \sum_{n=0}^\infty \frac{x^n}{n!},\qquad d) \; \sum_{n=0}^\infty x^{2n}
\]
\end{problem}

\end{document}








\begin{center}
\begin{foldable}
\unfoldable{Here is a detailed, lecture style video on average value:}
\youtube{gRJTe1i1muo}
\end{foldable}
\end{center}



\begin{tikzpicture}
\node[inner sep=0pt] (bird) at (0,0)
    {\includegraphics[width=.25\textwidth]{bird.jpg}};
\node[inner sep=0pt] (spiral) at (5,0)
    {\includegraphics[width=.25\textwidth]{spiral.jpg}};
\node[inner sep=0pt] (taylor) at (5,-5)
    {\includegraphics[width=1\textwidth]{taylor.png}};
\draw[->,thick] (bird) -- (spiral.north west)
    node[midway,fill=white] {bird};
\draw[->,thick] (spiral.south west) -- (bird.south east)
    node[midway,fill=white] {spiral};    
\end{tikzpicture}




\begin{example} %example #15
Find $h'(x)$ if $h(x) = x^{\sin(x)}$.\\
We will use the fact that the exponential and logarithm functions are inverses,
\[e^{\ln(x)} = x,\]
and the exponent property of logarithms, 
\[\ln(x^n) = n\ln(x),\]
to rewrite $h(x)$.  We have 
\[h(x) = x^{\sin(x)} = e^{\ln(x^{\sin(x)})} = e^{\sin(x)\ln(x)}\]
and we can now compute $h'(x)$ using a combination of the chain rule and product rule.
We can write $h(x)$ as a composition, $f(g(x))$ with 
\[g(x) = \sin(x)\ln(x) \quad \text{and} \quad f(x) = e^x.\]
Then to find $g'(x)$ we us the product rule and we get $g'(x) = \frac{\sin(x)}{x} + \cos(x)\ln(x)$.
Next $f'(x) = e^x$ and 
hence $f'(g(x)) = e^{g(x)} = e^{\sin(x)\ln(x)} = x^{\sin(x)}$.
We can then conclude $h'(x) = f'(g(x))g'(x) = x^{\sin(x)} \left[ \frac{\sin(x)}{x} + \cos(x)\ln(x)\right]$.
\end{example}

%more question formats below













%\begin{verbatim}
\begin{question}
What is your favorite color?
\begin{multipleChoice}
\choice[correct]{Rainbow}
\choice{Blue}
\choice{Green}
\choice{Red}
\end{multipleChoice}
\begin{freeResponse}
Hello
\end{freeResponse}
\end{question}
%\end{verbatim}





\begin{question}
  Which one will you choose?
  \begin{multipleChoice}
    \choice[correct]{I'm correct.}
    \choice{I'm wrong.}
    \choice{I'm wrong too.}
  \end{multipleChoice}
\end{question}


\begin{question}
  Which one will you choose?
  \begin{selectAll}
    \choice[correct]{I'm correct.}
    \choice{I'm wrong.}
    \choice[correct]{I'm also correct.}
    \choice{I'm wrong too.}
  \end{selectAll}
\end{question}


\begin{freeResponse}
What is the chain rule used for?
\end{freeResponse}
