\documentclass{ximera}

\input{../preamble}

\outcome{Compute definite integrals involving infinity}

\title{Improper Integrals}

\begin{document}

\begin{abstract}
We will compute definite integrals involving infinity.
\end{abstract}

\maketitle

\section{Introduction}
In this section we will consider definite integrals involving infinity.
There are two fundamentally different types of improper integrals.  The first involves infinity as an ``endpoint"
of integration and the second involves vertical asymptotes at or between the endpoints of integration.
Examples of the first type include
\[
\int_0^\infty e^{-2x} \; dx, \; \text{ and } \;  \int_{-\infty}^\infty \frac{1}{1+x^2}\; dx.
\]
The second of the above examples is called ``doubly improper" since it involves both $\infty$ and $-\infty$.
Examples of the second type include
\[
\int_0^{\pi/2} \tan(x)\; dx \; \text{ and } \; \int_0^1 \frac{1}{x} \; dx.
\]
If the value of an improper integral is a finite number, then we say that the integral \textbf{converges}.
Otherwise, we say that the integral \textbf{diverges}.
The method of computing improper integrals involves replacing an endpoint with a variable 
and then taking an appropriate limit as we will see in the examples below.




\section{Infinity as an endpoint}
\begin{definition}[Type 1 Improper Integral]
Suppose $f(x)$ is continuous on the interval $[a, \infty)$. Then we compute the improper integral at infinity as follows:
\[
\int_a^\infty f(x) \; dx = \lim_{b \to \infty} \int_a^b f(x) \; dx.
\]
The improper integral at negative infinity is defined similarly.
\end{definition}


\begin{example}
Compute the improper integral
\[
\int_0^\infty e^{-2x} \; dx.
\]

We will begin by replacing $\infty$ in the improper integral with the variable $b$, a typical choice for an upper endpoint of integration.
We compute
\begin{align*}
\int_0^b e^{-2x} \; dx &= \left(-\frac12 e^{-2x} \right) \bigg|_0^b\\
                       &= \left(-\frac12 e^{-2b} \right) - \left(-\frac12 e^{0} \right)\\
                       &=\frac12 -\frac12 e^{-2b}.
\end{align*}
                       
To complete the problem, we now take a limit as $b \to \infty$.
\begin{align*}
\int_0^\infty e^{-2x} \; dx &= \lim_{b \to \infty}\int_0^b e^{-2x} \; dx\\
                       &=\lim_{b \to \infty} \left(\frac12 -\frac12 e^{-2b}\right)\\
                       &= \frac12 -\frac12 e^{-\infty}\\
                       &= \frac12 - 0 \\
                       &= \frac12.
\end{align*}
Since the answer is a finite number we say that the integral converges.
More precisely, we can say that the integral converges to $1/2$.

\end{example}




\begin{problem}
Compute the improper integral
\[
\int_0^\infty 2e^{-5x} \; dx = \answer{2/5}
\]

\end{problem}






\begin{example}
Compute the improper integral
\[
\int_1^\infty \frac{3}{x^2} \; dx.
\]

We will begin by replacing $\infty$ in the improper integral with the variable $b$, a typical choice for an upper endpoint of integration.
We compute
\begin{align*}
\int_1^b \frac{3}{x^2} \; dx &= \int_1^b 3x^{-2} \; dx\\
                           &= \left(3\cdot \frac{x^{-1}}{-1} \right) \bigg|_1^b\\
                           &= \left(-\frac{3}{x} \right) \bigg|_1^b\\
                       &= \left(-\frac{3}{b} \right) - \left(-\frac{3}{1} \right)\\
                       &=3 - \frac{3}{b}.
\end{align*}
                       
To complete the problem, we now take a limit as $b \to \infty$.
\begin{align*}
\int_1^\infty \frac{3}{x^2} \; dx &= \lim_{b \to \infty}\int_1^b \frac{3}{x^2} \; dx\\
                       &=\lim_{b \to \infty} \left(3 - \frac{3}{b}\right)\\
                       &= 3 -\frac{3}{\infty}\\
                       &= 3 - 0 \\
                       &= 3.
\end{align*}
Since the answer is a finite number we say that the integral converges.
More precisely, we can say that the integral converges to $3$.

\end{example}



\begin{problem}
Compute the improper integral
\[
\int_2^\infty \frac{5}{x^3} \; dx = \answer{5/8}
\]

\end{problem}




\begin{example}
Compute the improper integral
\[
\int_1^\infty \frac{4}{x} \; dx.
\]

We will begin by replacing $\infty$ in the improper integral with the variable $b$, a typical choice for an upper endpoint of integration.
We compute
\begin{align*}
\int_1^b \frac{4}{x} \; dx &= \int_1^b \frac{4}{x} \; dx\\
                           &= \left(4\ln|x| \right) \bigg|_1^b\\
                       &= \left(4\ln|b| \right) - \left(4\ln|1| \right)\\
                       &=4\ln|b|.
\end{align*}
                       
To complete the problem, we now take a limit as $b \to \infty$.
\begin{align*}
\int_1^\infty \frac{4}{x} \; dx &= \lim_{b \to \infty}\int_1^b \frac{4}{x} \; dx\\
                       &=\lim_{b \to \infty} 4\ln|b|\\
                       &= 4\ln(\infty)\\
                       &= \infty.
\end{align*}
Since the answer is a \textbf{not} a finite number we say that the integral diverges.

\end{example}


\begin{problem}
Show that the improper integral diverges:
\[
\int_3^\infty \frac{7}{\sqrt x}.
\]
\end{problem}

Based on the previous examples and problems, we can expect the following theorem about integrals of the form
\[
\int_1^\infty \frac{1}{x^p} \; dx.
\]

\begin{theorem}[p-integrals]
The improper p-integral $\int_1^\infty \frac{1}{x^p} \; dx$
 converges if $p>1$ and diverges if $p \leq 1$
The result is the same if lower endpoint is replaced by any other positive number.
\end{theorem}
This theorem will be of value to us in future sections, but for now, we use it to help us with another improper integral.


\begin{example}
Compute the improper integral
\[
\int_2^\infty \frac{1}{x\ln(x)} \; dx.
\]
Using a u-substitution with $u = \ln(x)$ and $du = \frac{1}{x} \, dx$, the integral becomes
\[
\int_2^\infty \frac{1}{x\ln(x)} \; dx = \int_{\ln(2)}^\infty \frac{1}{u} \; du.
\]
This is a $p$-integral in the variable $u$ with $p=1$. Since $p \leq 1$, the theorem says that this integral diverges, and hence
\[
\int_2^\infty \frac{1}{x\ln(x)} \; dx \;\; \text{ diverges}.
\]
\end{example}



\section{Type 2 Improper Integrals}

In this section we examine definite integrals in which the integrand has a vertical asymptote at an endpoint of integration.

\begin{definition}[Type 2 Improper Integral]
Suppose $f(x)$ is continuous on the interval $(a, b]$ and that $f(x)$ has a vertical asymptote at $x = a$.
Then
\[
\int_a^b f(x) \; dx = \lim_{t \to a^+} \int_t^b f(x) \; dx.
\]
The improper integral is defined similarly if the vertical asymptote is at the upper endpoint of integration.
\end{definition}

\begin{example}
Compute the improper integral
\[
\int_0^1 \frac{3}{\sqrt x} \; dx.
\]
The integral is improper because the integrand has a vertical asymptote at $x = 0$. Hence
\begin{align*}
\int_0^1 \frac{3}{\sqrt x} \; dx &= \lim_{a \to 0^+} \int_a^1 \frac{3}{\sqrt x} \; dx\\
                                 &= \lim_{a \to 0^+} \int_a^1 3x^{-1/2} \; dx\\
                                 &= \lim_{a \to 0^+} \left( 6x^{1/2}  \right) \bigg|_a^1\\
                                 &= \lim_{a \to 0^+} \left( 6\sqrt{1} - 6\sqrt{a}  \right) \\
                                 &= \left( 6 - 6\sqrt{0}  \right) \\
                                 &= 6.
\end{align*}
 Hence the improper integral converges to 6.
 \end{example}
 
\begin{problem}
Compute the improper integral
\[
\int_2^6 \frac{4}{\sqrt{x-2}} \; dx = \answer{16}
\]
\end{problem}

                                 
\begin{center}
\begin{foldable}
\unfoldable{Here is a detailed, lecture style video on improper integrals:}
\youtube{gRJTe1i1muo}
\end{foldable}
\end{center}





\end{document}


\begin{example} %example #15
Find $h'(x)$ if $h(x) = x^{\sin(x)}$.\\
We will use the fact that the exponential and logarithm functions are inverses,
\[e^{\ln(x)} = x,\]
and the exponent property of logarithms, 
\[\ln(x^n) = n\ln(x),\]
to rewrite $h(x)$.  We have 
\[h(x) = x^{\sin(x)} = e^{\ln(x^{\sin(x)})} = e^{\sin(x)\ln(x)}\]
and we can now compute $h'(x)$ using a combination of the chain rule and product rule.
We can write $h(x)$ as a composition, $f(g(x))$ with 
\[g(x) = \sin(x)\ln(x) \quad \text{and} \quad f(x) = e^x.\]
Then to find $g'(x)$ we us the product rule and we get $g'(x) = \frac{\sin(x)}{x} + \cos(x)\ln(x)$.
Next $f'(x) = e^x$ and 
hence $f'(g(x)) = e^{g(x)} = e^{\sin(x)\ln(x)} = x^{\sin(x)}$.
We can then conclude $h'(x) = f'(g(x))g'(x) = x^{\sin(x)} \left[ \frac{\sin(x)}{x} + \cos(x)\ln(x)\right]$.
\end{example}

%more question formats below













%\begin{verbatim}
\begin{question}
What is your favorite color?
\begin{multipleChoice}
\choice[correct]{Rainbow}
\choice{Blue}
\choice{Green}
\choice{Red}
\end{multipleChoice}
\begin{freeResponse}
Hello
\end{freeResponse}
\end{question}
%\end{verbatim}





\begin{question}
  Which one will you choose?
  \begin{multipleChoice}
    \choice[correct]{I'm correct.}
    \choice{I'm wrong.}
    \choice{I'm wrong too.}
  \end{multipleChoice}
\end{question}


\begin{question}
  Which one will you choose?
  \begin{selectAll}
    \choice[correct]{I'm correct.}
    \choice{I'm wrong.}
    \choice[correct]{I'm also correct.}
    \choice{I'm wrong too.}
  \end{selectAll}
\end{question}


\begin{freeResponse}
What is the chain rule used for?
\end{freeResponse}
