\documentclass{ximera}

\input{../preamble}

\outcome{Solve separable differential equations}

\title{1.6 Separable Differential Equations}

\begin{document}

\begin{abstract}
We solve separable differential equations and initial value problems.
\end{abstract}

\maketitle

\section{Differential Equations}

A differential equation is an equation that involves one or more derivatives of an unknown function. 
Solving a differential equation entails determining the unknown function.

\begin{example}[example 1]
Solve the differential equation $y' = y$.\\
We seek $y = f(x)$ such that $f'(x) = f(x)$. By inspection $y = e^x$ is a solution of this equation.
However, $y = 2e^x$ is also a solution. In fact, there are infinitely many solutions: $y = Ce^x$,
where $C$ is any constant (including 0).
\end{example}

An initial value problem is a differential equation along with other information about the solution, usually the value of the function at a point.
The purpose of the initial value is to determine one specific solution of the differential equation, in the event that there was more than one solution.

\begin{example}[example 2]
Solve the initial value problem $y' = y, y(0) = 4$.\\
We saw in the last example that the differential equation $y' = y$ has infinitely many solutions, $y = Ce^x$, where $C$ is any constant.
The initial value $y(0) = 4$ can be used to determine the value of $C$ so that we will have a unique solution. Since $y(0) = Ce^0 = 4$, we can see that $C = 4$.
Thus the initial value problem $y' = y, y(0) = 4$ has the unique solution $y = 4e^x$.
\end{example}



\section{Separable Differential Equations}

A \textbf{separable differential equation} is a differential equation that can be put in the form
$y' = f(y)g(x)$. To solve such an equation, we rewrite $y'$ as $\frac{dy}{dx}$ and we move the $y$'s and the $dy$ to one 
side of the equation and the $x$'s and the $dx$ to the other. Then we integrate both sides and solve for $y$.

\begin{example}[example 3]
Solve the differential equation $y' = xy^2$.\\
Rewrite the equation as 
\[
\frac{dy}{dx} = xy^2.
\]
Move the $y^2$ to the left and the $dx$ to the right to get
\[
\frac{1}{y^2} \, dy = x \,  dx.
\]
Integrate both sides:
\[
\int \frac{1}{y^2}\,  dy  = \int x \, dx.
\]
This gives
\[
-\frac{1}{y} = \frac{x^2}{2} + C.
\]
Solve for $y$:
\[
\frac{1}{y} = -\frac{x^2}{2} + C
\]
Note that $-C$ has been replaced by $+C$, as this makes no difference. Now take reciprocals:
\[
y = \frac{1}{-\frac{x^2}{2} + C} = - \frac{2}{x^2 + C}.
\]
Note that $-2C$ was replaced by $+C$ as this makes no difference.
We can check the differential equation by calculating $y'$ and observing that $y = xy^2$.
From the quotient rule, we have
\[
y' = \frac{(x^2 + C)\cdot 0 - (-2)(2x)}{(x^2 + C)^2} = \frac{4x}{(x^2 + C)^2} 
\]
\[
= x \cdot \frac{4}{(x^2 + C)^2} = x \cdot \left[\frac{2}{x^2 + C}\right]^2 = xy^2.
\]



\end{example}




\begin{example}[example 4]
Solve the differential equation $y' = x^2y$.\\
Rewrite the equation as 
\[
\frac{dy}{dx} = x^2y.
\]
Move the $y$ to the left and the $dx$ to the right to get
\[
\frac{1}{y} \, dy = x^2 \,  dx.
\]
Integrate both sides:
\[
\int \frac{1}{y}\,  dy  = \int x^2 \, dx.
\]
This gives
\[
\ln|y| = \frac{x^3}{3} + C.
\]
Solve for $y$:
\[
|y| = e^{\frac{x^3}{3} + C} = e^C \cdot e^{x^3/3}.
\]
Note that $e^C$ is a positive constant. Remove the absolute values:
\[
y = \pm e^C \cdot e^{x^3/3} = Ae^{x^3/3},
\]
where $A$ is any non-zero constant. Looking back at the original differential equation, we see that $y = 0$ is a solution, so 
we can say that $A$ is actually any constant.
We can check the differential equation by calculating $y'$ and observing that $y = x^2y$.
From the chain rule, we have
\[
y' = Ae^{x^3/3}\cdot \frac{d}{dx} \frac{x^3}{3} = Ae^{x^3/3} \cdot x^2 = x^2 y.
\]

\end{example}



\begin{example}[example 5]
A population of 2 million bacteria doubles in 1 hour. If we assume that the population is growing at a rate which is proportional to the number of bacteria present,
write a differential equation that models the population at time $t$ and find the population after 90 minutes.\\
Let $P = P(t)$ denote the population of the bacteria (in millions) after $t$ hours.
Since the rate of growth is proportional to the number present, we have
\[
\frac{dP}{dt} = k P,
\]
for some constant $k$.
Moving $P$ to the left and $dt$ to the right and integrating gives
\[
\int \frac{1}{P}\, dP = \int k \, dt
\]
Anti-differentiating gives:
\[
\ln|P| = kt + C
\]
Solving for $P$:
\[
|P| = e^{kt+C} = e^C \cdot e^{kt},
\]
Removing the absolute value bars, we have
\[
P = \pm e^C \cdot e^{kt} = Ae^{kt},
\]
where $A$ is a nonzero constant.
To determine the values of $A$ and $k$ we will use the given information about the size of the population at time $t = 0$ and $t = 1$.
The population was initially 2 million, so $P(0) = 2$ and in one hour it doubled, so $P(1) = 4$. the first of these gives,
\[
P(0) = Ae^{0} = 2 \implies A = 2.
\]
Using the second condition gives:
\[
P(1) = 2e^k = 4 \implies e^k = 2 \implies k = \ln(2).
\]
Thus $P(t) = 2e^{\ln(2)t}$ is the formula for the population at time $t$. Finally, after 90 minutes (or 1.5 hours), the population is 
$P(1.5) = 2e^{1.5\ln(2)} \approx 5.66$ million bacteria.

\end{example}








\end{document}



%more question formats below













%\begin{verbatim}
\begin{question}
What is your favorite color?
\begin{multipleChoice}
\choice[correct]{Rainbow}
\choice{Blue}
\choice{Green}
\choice{Red}
\end{multipleChoice}
\begin{freeResponse}
Hello
\end{freeResponse}
\end{question}
%\end{verbatim}





\begin{question}
  Which one will you choose?
  \begin{multipleChoice}
    \choice[correct]{I'm correct.}
    \choice{I'm wrong.}
    \choice{I'm wrong too.}
  \end{multipleChoice}
\end{question}


\begin{question}
  Which one will you choose?
  \begin{selectAll}
    \choice[correct]{I'm correct.}
    \choice{I'm wrong.}
    \choice[correct]{I'm also correct.}
    \choice{I'm wrong too.}
  \end{selectAll}
\end{question}


\begin{freeResponse}
What is the chain rule used for?
\end{freeResponse}
