\documentclass{ximera}

\input{../preamble}
\usetikzlibrary{matrix,positioning}

\outcome{Compute an integral using integration by parts}

\title{Integration by Parts}

\begin{document}

\begin{abstract}
We will compute integrals using the integration by parts technique.
\end{abstract}

\maketitle

%\begin{center}
%\textbf{Integration by Parts}
%\end{center}

We will use the integration by parts (IBP) formula to compute integrals involving products of unrelated factors.


\begin{theorem}[Integration by Parts]
\[
\int u \; dv = uv - \int v \; du
\]
\end{theorem}

\begin{remark}
The integration by Parts formula does not give a final answer to a problem. 
Instead, it replaces one integral with another, which still has to be solved.
The goal is for this new integral to be easier than the original one.
\end{remark}




\begin{example} %example #1
Compute the integral using IBP:
  \[
  \int x\sin(x) \;dx.
  \]
  
  The integrand is the product of two factors, $x$ and $\sin(x)$.  We consider one factor to differentiate and the other factor to anti-differentiate.
  The factor we prefer to differentiate is $x$ since the derivative of $x$ is a constant and constants are easy to deal with in integrals.
  As for the $\sin(x)$ factor, whether we differentiate it or anti-differentiate it makes little difference.  In fact, only a change in sign occurs,
  as 
  \[\frac{d}{dx}{\sin(x)} = \cos(x) \;\;  \text{ and }\;\;   \int \sin(x) \;dx = -\cos(x) + C.\]
  Thus to apply the IBP formula, we let
  \[u=x \text{  and  }  dv = \sin(x) \;dx.\]
  Next, we compute
  \[du = dx  \;\;  \text{  and  }\;\;    v = -\cos(x).\]
  \begin{remark} 
  We do not need to add the constant of integration to v, as any anti-derivative will suffice 
  for our purpose and we choose the constant of integration to be zero.
  \end{remark}
  Now we use the Integration by Parts formula, $\int u\;dv = uv-\int v\; du$:
  \begin{align*}
  \int x\sin(x) &= \overbrace{x}^{u}\overbrace{[-\cos(x)]}^{v} - \int \overbrace{-\cos(x)}^{v} \;\overbrace{dx}^{du}\\
                &= -x\cos(x) + \int \cos(x) \;dx\\
                &= -x\cos(x) + \sin(x) + C.
 \end{align*}
 
  We have found an answer, but at this stage we should prove that it is the correct answer by differentiating it.  The result should be $x\sin(x)$.
  Note that the differentiation requires the product rule on the $uv$ term: $-x\cos(x)$.
  We have
  \[
  \frac{d}{dx}{\left[-x\cos(x) + \sin(x) + C\right]} = [-\cos(x) + x\sin(x)] + \cos(x) = x\sin(x)
  \]
  which proves that our answer was correct.
  
    
\end{example}

\begin{center}
\begin{foldable}
\unfoldable{Here is a video of Example 1}
%\youtube{Yy6QXnFlnXs} %vid of example 1
\end{foldable}
\end{center}


\begin{problem} %problem #1
  Compute the integral using IBP:
  \[
  \int xe^x \;dx.
  \]
  
  Let $u = \answer{x}$   and   $dv = \answer{e^x dx}$.\\
  Then $du = \answer{dx}$   and   $v = \answer{e^x}$.\\
  Thus 
  \[
  \int xe^x dx = xe^x - \int \answer{e^x} dx = \answer{xe^x - e^x} + C.
  \]
  


  %\begin{hint}
   %   $\int udv = uv-\int vdu$
  %\end{hint}
    

\end{problem}


\begin{problem} %problem #1
  Compute the integral using IBP:
  \[
  \int x\cos(x) \;dx.
  \]
  
  Let $u = \answer{x}$   and   $dv = \answer{\cos(x) \;dx}$.\\
  Then $du = \answer{dx}$   and   $v = \answer{\sin(x)}$.\\
  Thus 
  \[
  \int x\cos(x) dx = x\sin(x) - \int \answer{\sin(x)} \;dx = \answer{x\sin(x) + \cos(x)} + C.
  \]
  


  %\begin{hint}
   %   $\int udv = uv-\int vdu$
  %\end{hint}
    

\end{problem}


\begin{example}
Compute the integral using IBP:
  \[
  \int 3x\sin(4x) \;dx.
  \]

Let $u = 3x$ and $dv = \sin(4x) \,dx$.\\
Then $du = 3 \,dx$ and $v = -\frac14 \cos(4x)$.
Next, the IBP formula gives
\begin{align*}
  \int 3x\sin(4x) \;dx &= \overbrace{3x}^{u}\overbrace{\left[-\frac14 \cos(4x)\right]}^{v} - \int \overbrace{-\frac14 \cos(4x)}^{v}  \cdot \overbrace{3 \; dx}^{du} \\
                       &= -\frac34 x\cos(4x) + \frac34 \int \cos(4x) \; dx \\
                       &= -\frac34 x\cos(4x) + \frac34 \cdot \frac 14 \sin(4x) + C\\
                       &= -\frac34 x\cos(4x) + \frac{3}{16}\sin(4x) + C.
\end{align*}

\end{example}


\begin{problem}
Compute the integral using IBP:
  \[
  \int 2x\sin(5x)\;dx.
  \]

\end{problem}


\begin{problem}
Compute the integral using IBP:
  \[
  \int 6xe^{-3x} \;dx.
  \]

\end{problem}


\begin{problem}
Compute the integral using IBP:
  \[
  \int x\sin(x/2) \;dx.
  \]

\end{problem}


\begin{example}[IBP twice]
Compute the integral using IBP:
  \[
  \int x^2\sin(3x) \;dx.
  \]

\[
\text{Let} \;\; u = x^2 \;\; \text{and} \;\; dv = \sin(3x) \,dx,
\]
\[
\text{then} \;\; du = 2x \,dx \;\; \text{and} \;\; v = -\frac13 \cos(3x).
\]

Next, the IBP formula gives
\begin{align*}
\int x^2\sin(3x) \;dx &= x^2\left[-\frac13 \cos(3x)\right] - \int -\frac13 \cos(3x) \cdot 2x \; dx \\
                       &= -\frac13 x^2\cos(3x) + \frac13 \int 2x\cos(3x) \; dx\\                               
\text{we now use IBP} & \text{ again with } \;\; u = 2x \;\text{ and } \; dv = \cos(3x) \, dx\\
& \qquad \qquad \quad du = 2 \, dx \; \text{ and } \; v=\frac13 \sin(3x)\\
                       &= -\frac13 x^2\cos(3x) + \frac29x\sin(3x) - \frac13 \int \frac13 \sin(3x)\cdot 2 \; dx\\
                       &= -\frac13 x^2\cos(3x) + \frac29x\sin(3x) + \frac{2}{27} \cos(3x) + C.
\end{align*}

\end{example}


\begin{problem}
Compute the integral using IBP:
  \[
  \int x^2\cos(2x) \;dx.
  \]

\end{problem}

\begin{problem}
Compute the integral using IBP:
  \[
  \int x^2e^{-x} \;dx.
  \]

\end{problem}

\begin{center}
\textbf{Tabular Integration}
\end{center}

Integrals of the form $\int x^n f(x) \,dx$ require IBP $n$ times when $f(x)$ is a sine, cosine or exponential function.
A notational shortcut called \textbf{tabular integration} can be used to streamline the process of using IBP multiple times.
As an example, let's revisit the previous example:

\begin{example}[Tabular Integration]
Compute the integral using tabular integration:
  \[
  \int x^2\sin(3x) \;dx.
  \]

We will construct a table that lists the derivatives of $u$ and the anti-derivatives of $dv$.
We can then obtain the final answer by a series of multiplications and additions or subtractions, as indicated
by the arrows in the table.


\begin{image}[5cm]
\begin{tikzpicture}
 \matrix (m) [matrix of nodes, ampersand replacement=\&,
            column sep = 1.5cm]{
    u     \&                  dv \\\hline
    $x^2$ \& $\sin(3x)$ \\ [8pt]
     $2x$  \& $-\frac13\cos(3x)$ \\ [8pt]
      $2$ \& $-\frac19\sin(3x)$ \\ [8pt]
       $0$ \& $\frac{1}{27}\cos(3x)$ \\
 };
 \draw[-latex] (m-2-1) -- (m-3-2) node[midway,above]{$+$};  % <-- It works!
 \draw[-latex] (m-3-1) -- (m-4-2) node[midway,above]{$-$};  % <-- It works!
 \draw[-latex] (m-4-1) -- (m-5-2) node[midway,above]{$+$};  % <-- It works!
 %\node at (-.6, 1.5){$+$};
 %\node at (-.6, 0.3){$-$};
 %\node at (-.6, -0.9){$+$};
 %\draw (,) -- (,);
\end{tikzpicture}
\end{image}

Thus,
\[
  \int x^2\sin(3x) \;dx = -\frac13 x^2\cos(3x) + \frac29x\sin(3x) + \frac{2}{27} \cos(3x) + C.
  \]

\end{example}



\begin{example}[Tabular Integration]
Compute the integral using Tabular Integration:
  \[
  \int x^4 e^{-2x} \;dx.
  \]
We construct a table with the derivatives of $u = x^4$ and the anti-derivatives of $dv = e^{-2x} \, dx$.
We add arrows which indicate multiplication of an element of the $u$ column with elements in the $dv$ column one row lower.
We adorn the arrows with alternating $+$ and $-$ signs to indicate either addition or subtraction of terms.
\begin{image}[5cm]
\begin{tikzpicture}
 \matrix (m) [matrix of nodes, ampersand replacement=\&,
            column sep = 1.5cm]{
    u     \&                  dv \\\hline
    $x^4$ \& $e^{-2x}$ \\ [8pt]
     $4x^3$  \& $-\frac12 e^{-2x}$ \\ [8pt]
      $12x^2$ \& $\frac14 e^{-2x}$ \\ [8pt]
       $24x$ \& $-\frac18 e^{-2x}$ \\[8pt]
       $24$ \& $\frac{1}{16} e^{-2x}$ \\[8pt]
       $0$ \& $-\frac{1}{32} e^{-2x}$ \\
 };
 \draw[-latex] (m-2-1) -- (m-3-2) node[midway,above]{$+$};  % <-- It works!
 \draw[-latex] (m-3-1) -- (m-4-2) node[midway,above]{$-$};  % <-- It works!
 \draw[-latex] (m-4-1) -- (m-5-2) node[midway,above]{$+$};  % <-- It works!
 \draw[-latex] (m-5-1) -- (m-6-2) node[midway,above]{$-$};  % <-- It works!
 \draw[-latex] (m-6-1) -- (m-7-2) node[midway,above]{$+$};  % <-- It works!
 %\node at (-.6, 1.5){$+$};
 %\node at (-.6, 0.3){$-$};
 %\node at (-.6, -0.9){$+$};
 %\draw (,) -- (,);
\end{tikzpicture}
\end{image}

Thus,
\[
  \int x^4 e^{-2x} \;dx = -\frac12 x^4 e^{-2x} - \frac44x^3 e^{-2x} - \frac{12}{8} x^2 e^{-2x} - \frac{24}{16}x e^{-2x} - \frac{24}{32} e^{-2x} + C.
  \]
\[
= \left(-\frac12 x^4 - x^3  - \frac{3}{2} x^2  - \frac{3}{2}x  - \frac{3}{4}\right) e^{-2x} + C.
\]
\end{example}


\begin{problem}[Tabular Integration]
Compute the integral using Tabular Integration:
  \[
  \int x^3 \cos(5x) \;dx.
  \]
Complete the table and then enter the final answer.
\begin{center}
\[
\begin{array}{c|c}
		u & dv  \\\hline 
		x^3 & \cos(5x) \\ 
     \answer{3x^2} & \answer{\frac15 \sin(5x)} \\ 
      \answer{6x} & \answer{-\frac{1}{25} \cos(5x)} \\ 
       \answer{6} & \answer{-\frac{1}{125} \sin(5x)} \\
       0 & \answer{\frac{1}{625} \cos(5x)} 
	\end{array}
    \]
\end{center}



Thus,
\[
  \int x^3 \cos(5x) \;dx = \answer{\frac15 x^3\sin(5x) + \frac{3}{25}x^2 \cos(5x) - \frac{6}{125}\sin(5x) -\frac{6}{625}\cos(5x)} +C.
  \]
\end{problem}



\begin{center}
\textbf{Inverse Functions}
\end{center}
We will now look at some examples involving inverse functions like $\ln(x), \tan^{-1}(x), \sin^{-1}(x)$ and $\cos^{-1}(x)$.
We do not (yet) know anti-derivatives for these functions, so we will have to let $u$ equal the inverse function.
 
\begin{example}
Compute the integral using IBP:
  \[
  \int x^5\ln(x) \;dx.
  \]
In our previous examples, we would have let $u = x^5$ and $dv = \ln(x) \, dx$.
But notice that,in this case, we do not know an anti-derivative of $\ln(x)$, so 
we would be stumped in finding $v$. Instead, we will let 
\[
u = \ln(x)  \text{  and  } dv = x^5 \, dx\]
then
\[
du = \frac{1}{x} \, dx \text{  and  } v = \frac{x^6}{6}.
\]
The power of $x$ has increased, rather than decreased, as in previous examples, but this 
is offset by the fact that the derivative of the natural log has a completely different form
which is easier to work with. Now, by IBP, we have,

\begin{align*}
  \int x^5\ln(x) \;dx &= \frac{x^6}{6}\ln(x) - \int \frac{x^6}{6}\cdot \frac{1}{x} \, dx\\
\text{Now, the integrand } & \text{ can be simplified by canceling $x$ allowing us to integrate}\\
&= \frac{x^6}{6}\ln(x) - \frac16\int x^5 \, dx\\
&= \frac{x^6}{6}\ln(x) -  \frac{x^6}{36} + C\\
\end{align*}

\end{example}



\begin{problem} 
  Compute the integral using IBP:
  \[
  \int x^8 \ln(x) \;dx.
  \]
  
  \begin{hint}
      include $dx$ where appropriate
  \end{hint}
  Let $u = \answer{\ln(x)}$   and   $dv = \answer{x^8 \;dx}$.\\
  Then $du = \answer{\frac{1}{x} dx}$   and   $v = \answer{x^9/9}$.\\
  Thus 
  \[
  \int x^8 \ln(x) dx = \frac{x^9}{9}\ln(x) - \int \answer{\frac{x^8}{9}} \;dx = \answer{\frac{x^9}{9}\ln(x) -\frac{x^9}{81}} + C.
  \]

\end{problem}

This method can be used to anti-differentiate $\ln(x)$ as well.


\begin{problem} 
  Compute the integral using IBP:
  \[
  \int \ln(x) \;dx.
  \]
  
  \begin{hint}
      include $dx$ where appropriate
  \end{hint}
  Let $u = \answer{\ln(x)}$   and   $dv = \answer{dx}$.\\
  Then $du = \answer{\frac{1}{x} dx}$   and   $v = \answer{x}$.\\
  Thus 
  \[
  \int  \ln(x) dx = x\ln(x) - \int \answer{1} \;dx = \answer{x\ln(x) -x} + C.
  \]

\end{problem}

\begin{problem} 
  Compute the integral using IBP:
  \[
  \int \frac{\ln(x)}{\sqrt x} \;dx.
  \]
  
  \begin{hint}
      include $dx$ where appropriate
  \end{hint}
  \begin{hint}
      rewrite $\frac{1}{\!\sqrt x}$ as a power of $x$
  \end{hint}
  Let $u = \answer{\ln(x)}$   and   $dv = \answer{x^{-1/2} \;dx}$.\\
  Then $du = \answer{\frac{1}{x} dx}$   and   $v = \answer{2x^{1/2}}$.\\
  Thus 
  \[
  \int \frac{\ln(x)}{\!\sqrt x} dx = 2\sqrt x \ln(x) - \int \answer{\frac{2}{\sqrt x}} \;dx = \answer{2\sqrt x \ln(x) -4\sqrt x} + C.
  \]

\end{problem}


\begin{example}
Compute the integral:
  \[
  \int \tan^{-1}(2x) \;dx.
  \]
Let $u = \tan^{-1}(2x)$   and   $dv = dx$.\\
  Then $du = \frac{2}{1+4x^2}\, dx$   and   $v = x$.\\
By IBP,
  \begin{align*}
  \int  \tan^{-1}(2x) dx &= x\tan^{-1}(2x) - \int \frac{2x}{1+4x^2} \;dx\\
  \text{we can use $u$-} & \text{substitution on this integral} \\
  \text{with $u =$} &  1+4x^2 \text{ and } du = 8x \, dx \\
  &= x\tan^{-1}(2x) - \frac14 \int \frac{1}{u} \; du\\
  &= x\tan^{-1}(2x) - \frac14 \ln|u| + C\\
  &= x\tan^{-1}(2x) - \frac14 \ln(1+4x^2) + C
  \end{align*}
  
\end{example}

\begin{problem}
Compute the integral:
  \[
  \int \tan^{-1}(x) \;dx.
  \]

\end{problem}

\begin{problem}
Compute the integral:
  \[
  \int \sin^{-1}(4x) \;dx.
  \]

\end{problem}

\begin{example}
Compute the integral:
  \[
  \int x^3\tan^{-1}(x) \;dx.
  \]
Let $u = \tan^{-1}(x)$   and   $dv = x^3 \, dx$.\\
  Then $du = \frac{1}{1+x^2}\, dx$   and   $v = \frac14 x^4$.\\
By IBP,
  \begin{align*}
  \int  \tan^{-1}(x) dx &= \frac14 x^4\tan^{-1}(x) - \frac14\int \frac{x^4}{1+x^2} \;dx\\
  & \text{now use polynomial long division to get} \\
  &= \frac14 x^4\tan^{-1}(x) - \frac14 \int x^2 - 1 + \frac{1}{1+x^2} \; dx\\
  &= \frac14 x^4\tan^{-1}(x) - \frac14\left(\frac{x^3}{3} - x + \tan^{-1}(x)\right) + C\\
  &= \frac14 x^4\tan^{-1}(x) - \frac{x^3}{12} - \frac{x}{4} + \frac14 \tan^{-1}(x) + C
  \end{align*}
  
\end{example}

\begin{problem}
Compute the integral:
  \[
  \int x^2\tan^{-1}(x) \;dx.
  \]
\begin{hint}
      include $dx$ where appropriate
  \end{hint}
  Let $u = \answer{\tan^{-1}(x)}$   and   $dv = \answer{x^2 \;dx}$.\\
  Then $du = \answer{\frac{1}{1+x^2} dx}$   and   $v = \answer{x^3/3}$.\\
  Thus 
  \[
  \int x^2 \tan^{-1}(x) \; dx = \frac13 x^3 \tan^{-1}(x) - \int \answer{\frac13 \frac{x^3}{1+x^2}} \;dx = 
  \answer{\frac13 x^3 \tan^{-1}(x) - \frac{x^2}{6} + \frac16\ln(1+x^2)} + C.
  \]
\end{problem}


%Other interesting examples: e^x cos(x), sec^3(x)
%gamma function
%reduction of powers

\begin{center}
\begin{foldable}
\unfoldable{Here is a detailed, lecture style video on integration by parts:}
\youtube{2jSr68xaAfs}
\end{foldable}
\end{center}





\end{document}











\begin{image}
\begin{tikzpicture}
 \matrix (m) [matrix of nodes, ampersand replacement=\&,
            column sep = 1.5cm]{
    u     \&                  dv \\\hline
    $x^3$ \& $\cos(5x)$ \\ [8pt]
     $\answer{3x^2}$  \& $\answer{\frac15 \sin(5x)}$ \\ [8pt]
      $\answer{6x}$ \& $\answer{-\frac{1}{25} \cos(5x)}$ \\ [8pt]
       $\answer{6}$ \& $\answer{-\frac{1}{125} \sin(5x)}$ \\[8pt]
       $0$ \& $\answer{\frac{1}{625} \cos(5x)}$\\     
 };
 \draw[-latex] (m-2-1) -- (m-3-2) node[midway,above]{$+$};  % <-- It works!
 \draw[-latex] (m-3-1) -- (m-4-2) node[midway,above]{$-$};  % <-- It works!
 \draw[-latex] (m-4-1) -- (m-5-2) node[midway,above]{$+$};  % <-- It works!
 \draw[-latex] (m-5-1) -- (m-6-2) node[midway,above]{$-$};  % <-- It works!
\end{tikzpicture}
\end{image}



\begin{example} %example #15
Find $h'(x)$ if $h(x) = x^{\sin(x)}$.\\
We will use the fact that the exponential and logarithm functions are inverses,
\[e^{\ln(x)} = x,\]
and the exponent property of logarithms, 
\[\ln(x^n) = n\ln(x),\]
to rewrite $h(x)$.  We have 
\[h(x) = x^{\sin(x)} = e^{\ln(x^{\sin(x)})} = e^{\sin(x)\ln(x)}\]
and we can now compute $h'(x)$ using a combination of the chain rule and product rule.
We can write $h(x)$ as a composition, $f(g(x))$ with 
\[g(x) = \sin(x)\ln(x) \quad \text{and} \quad f(x) = e^x.\]
Then to find $g'(x)$ we us the product rule and we get $g'(x) = \frac{\sin(x)}{x} + \cos(x)\ln(x)$.
Next $f'(x) = e^x$ and 
hence $f'(g(x)) = e^{g(x)} = e^{\sin(x)\ln(x)} = x^{\sin(x)}$.
We can then conclude $h'(x) = f'(g(x))g'(x) = x^{\sin(x)} \left[ \frac{\sin(x)}{x} + \cos(x)\ln(x)\right]$.
\end{example}

%more question formats below













%\begin{verbatim}
\begin{question}
What is your favorite color?
\begin{multipleChoice}
\choice[correct]{Rainbow}
\choice{Blue}
\choice{Green}
\choice{Red}
\end{multipleChoice}
\begin{freeResponse}
Hello
\end{freeResponse}
\end{question}
%\end{verbatim}





\begin{question}
  Which one will you choose?
  \begin{multipleChoice}
    \choice[correct]{I'm correct.}
    \choice{I'm wrong.}
    \choice{I'm wrong too.}
  \end{multipleChoice}
\end{question}


\begin{question}
  Which one will you choose?
  \begin{selectAll}
    \choice[correct]{I'm correct.}
    \choice{I'm wrong.}
    \choice[correct]{I'm also correct.}
    \choice{I'm wrong too.}
  \end{selectAll}
\end{question}


\begin{freeResponse}
What is the chain rule used for?
\end{freeResponse}
