\documentclass{ximera}

\input{../preamble}

\outcome{Determine series behavior based on a definite integral}

\title{Integral Test}

\begin{document}

\begin{abstract}
We determine the convergence or divergence of an infinite series using a related improper integral.
\end{abstract}

\maketitle

\section{Integral Test}

\begin{theorem}[Integral Test]
Suppose that the function $f(x)$ is continuous, positive, and decreasing on the interval $(1, \infty)$, and 
suppose that the terms of an infinite series
are given by the corresponding function values, i.e., $a_n = f(n)$. \\
Then the improper integral
\[
\int_1^\infty f(x) \; dx.
\]
and the associated infinite series
\[
\sum_{n=1}^\infty a_n
\]
both converge or both diverge. In other words, the behavior of the improper integral 
determines the behavior of the associated series.
\end{theorem}

\begin{example}
Determine whether the series
\[
\sum_{n=0}^\infty \frac{1}{1+n^2}
\]
converges or diverges.\\
Consider the function, $f(x) = \frac{1}{1+x^2}$, so that $a_n = f(n)$.
This function is positive and continuous on the interval $(0, \infty)$.
To see that the function is decreasing, we recall that if the derivative is negative then the function is decreasing.
Using the Quotient Rule, we can see that the derivative is given by 
\[
f'(x) = -\frac{2x}{(1+x^2)^2}.
\]
Since $f'(x)$ is negative on the interval $(0, \infty)$, the original function $f(x)$ is decreasing on that interval.
Hence the conditions of the Integral Test are met and the behavior of the series is determined by the behavior of the improper integral:
\begin{align*}
\int_0^\infty \frac{1}{1+x^2} \; dx &= \lim_{b \to \infty} \int_0^b \frac{1}{1+x^2} \; dx\\
&= \lim_{b \to \infty} \tan^{-1}(x) \bigg|_0^b \\
&= \lim_{b \to \infty} \left[\tan^{-1}(b) - \tan^{-1}(0)\right]\\
&= \lim_{b \to \infty} \left[\tan^{-1}(b)\right]\\
&= \frac{\pi}{2}.
\end{align*}
We see that the improper integral converges. By the Integral Test, the associated infinite series
\[
\sum_{n=0}^\infty \frac{1}{1+n^2}
\]
also converges.
\end{example}


\begin{definition}[p-series]
Let $p > 0$. The infinite series
\[
\sum_{n=1}^\infty \frac{1}{n^p}
\]
is called a \textbf{$p$-series}. In the special case $p = 1$, the series is known as the \textbf{harmonic series}.
\end{definition}

We have seen in the section on improper integrals that the $p$-integral

\[
\int_1^\infty \frac{1}{x^p} \; dx.
\]
converges if $p > 1$ and diverges if $p \leq 1$.
Since the function $f(x) = 1/x^p \; (p > 0)$ is continuous, positive, and decreasing on the interval $(1, \infty)$,
the integral test can be applied to conclude that the associated $p$-series has the same behavior.  This is stated in the following theorem.


\begin{theorem}[$p$-series]
The series
\[
\sum_{n=1}^\infty \frac{1}{n^p}
\]
converges if $p > 1$ and diverges if $p \leq 1$.
\end{theorem}


\section{Video Lesson}

\begin{center}
\begin{foldable}
\unfoldable{Here is a detailed, lecture style video on the Integral Test:}
\youtube{db7NqcbCO4w&t}
\end{foldable}
\end{center}



\section{More Problems}



\end{document}


\begin{example} %example #15
Find $h'(x)$ if $h(x) = x^{\sin(x)}$.\\
We will use the fact that the exponential and logarithm functions are inverses,
\[e^{\ln(x)} = x,\]
and the exponent property of logarithms, 
\[\ln(x^n) = n\ln(x),\]
to rewrite $h(x)$.  We have 
\[h(x) = x^{\sin(x)} = e^{\ln(x^{\sin(x)})} = e^{\sin(x)\ln(x)}\]
and we can now compute $h'(x)$ using a combination of the chain rule and product rule.
We can write $h(x)$ as a composition, $f(g(x))$ with 
\[g(x) = \sin(x)\ln(x) \quad \text{and} \quad f(x) = e^x.\]
Then to find $g'(x)$ we us the product rule and we get $g'(x) = \frac{\sin(x)}{x} + \cos(x)\ln(x)$.
Next $f'(x) = e^x$ and 
hence $f'(g(x)) = e^{g(x)} = e^{\sin(x)\ln(x)} = x^{\sin(x)}$.
We can then conclude $h'(x) = f'(g(x))g'(x) = x^{\sin(x)} \left[ \frac{\sin(x)}{x} + \cos(x)\ln(x)\right]$.
\end{example}

%more question formats below













%\begin{verbatim}
\begin{question}
What is your favorite color?
\begin{multipleChoice}
\choice[correct]{Rainbow}
\choice{Blue}
\choice{Green}
\choice{Red}
\end{multipleChoice}
\begin{freeResponse}
Hello
\end{freeResponse}
\end{question}
%\end{verbatim}





\begin{question}
  Which one will you choose?
  \begin{multipleChoice}
    \choice[correct]{I'm correct.}
    \choice{I'm wrong.}
    \choice{I'm wrong too.}
  \end{multipleChoice}
\end{question}


\begin{question}
  Which one will you choose?
  \begin{selectAll}
    \choice[correct]{I'm correct.}
    \choice{I'm wrong.}
    \choice[correct]{I'm also correct.}
    \choice{I'm wrong too.}
  \end{selectAll}
\end{question}


\begin{freeResponse}
What is the chain rule used for?
\end{freeResponse}
