\documentclass{ximera}

\input{../preamble}

\outcome{Learn the fundamental limit laws}

\title{1.4a Limit Laws}


\begin{document}

\begin{abstract}
Learn the fundamental limit laws.
\end{abstract}

\maketitle

\section{Limit Laws}
 
 In section 1.2, Numerical Limits, we briefly discussed ``plugging in" to compute limits.
 The example we investigated was
 \[
 \lim_{x \to 3+} \left(x^2 + 2 \right) = 3^2 + 2 = 11.
 \]
 The reason plugging in worked in the previous example was a direct consequence of the limit laws presented below.
 
In each of the following, all of the limits are assumed to exist.

\begin{enumerate}

\item[1.]  
The limit of a constant is the constant:
 \[
 \lim_{x \to c} k = k.
 \]
 
\item[2.]
 The next law is self-evident:
 \[
 \lim_{x \to c} x = c.
 \]
 
 \item[3.]
 The limit of a multiple of a function is the multiple of the limit:
 \[
 \lim_{x \to c} kf(x) = k \cdot \lim_{x \to c} f(x). 
 \]
 
 \item[4.]
 The limit of a sum is the sum of the limits:
 \[
 \lim_{x \to c} \left[f(x) + g(x) \right] = \lim_{x \to c} f(x) + \lim_{x \to c} g(x). 
 \]
 
\item[5.]
 The limit of a difference is the difference of the limits:
 \[
 \lim_{x \to c} \left[f(x) - g(x) \right] = \lim_{x \to c} f(x) - \lim_{x \to c} g(x). 
 \]
 
\item[6.]
 The limit of a product is the product of the limits:
 \[
 \lim_{x \to c} f(x) g(x) = \lim_{x \to c} f(x) \cdot \lim_{x \to c} g(x). 
 \]


\item[7.]
 The limit of a quotient is the quotient of the limits:
 \[
 \lim_{x \to c} \frac{f(x)}{g(x)} = \frac{\lim_{x \to c} f(x)}{\lim_{x \to c} g(x)}, 
 \]
 provided that the limit in the denominator is \textbf{not equal to zero}.
 
 \item[8.]
 Limits can be moved inside of radicals:
 \[
 \lim_{x \to c} \sqrt[n]{f(x)} = \sqrt[n]{\lim_{x \to c} f(x)}. 
 \]

\end{enumerate}


Each of the above limit laws is valid if $x \to c^+, x\to c^-, x \to \infty$ or $x \to -\infty$.


\section{Problems}

\begin{example}[example 1] Given that 
\[
\lim_{x \to 3} f(x) = -5 \quad \text{and} \quad \lim_{x \to 3} g(x) = \tfrac12,
\]
find 
\[
\lim_{x \to 3} \left[x^2f(x) - 6g(x)\right].
\]
Using limit laws 2, 3 and 5, we can write
\[
\lim_{x \to 3} \left[x^2f(x) - 6g(x)\right] = \lim_{x \to 3} x^2 \cdot \lim_{x \to 3}f(x) - 6\lim_{x \to 3} g(x) = 9(-5) - 6(\tfrac12) = -48.
\]
\end{example}


\begin{problem}(problem 1a)
Given that 
\[
\lim_{x \to -2} f(x) = 2 \quad \text{and} \quad \lim_{x \to -2} g(x) = 0,
\]
\[
\lim_{x \to -2} \left[3f(x) + xg(x)\right] = \answer{6}.
\]
\end{problem}


\begin{problem}(problem 1b)
Given that 
\[
\lim_{x \to 1^+} f(x) = \tfrac23 \quad \text{and} \quad \lim_{x \to 1+} g(x) = 4,
\]
\[
\lim_{x \to 1^+} \frac{f(x)}{\sqrt{g(x)}} = \answer{1/3}.
\]
\end{problem}


\begin{problem}(problem 1c)
Given that 
\[
\lim_{x \to \infty} f(x) = -9 \quad \text{and} \quad \lim_{x \to \infty} g(x) = 1,
\]
\[
\lim_{x \to \infty} \sqrt[3]{f(x) + g(x)} = \answer{-2}.
\]
\end{problem}




\end{document}
