\documentclass{ximera}

\input{../preamble}

\outcome{Determine the behavior of a Telescoping Series}

\title{Telescoping Series}

\begin{document}

\begin{abstract}
We determine the convergence or divergence of a Telescoping Series.
\end{abstract}

\maketitle

\section{Telescoping Series}

A telescoping series is a special type of series whose terms cancel each out in such a way that it is relatively easy to determine the
exact value of its partial sums. Creating the telescoping effect frequently involves a partial fraction decomposition.

\begin{example}[example 1]
Consider the series
\[
\sum_{n=1}^\infty \frac{1}{n^2 +n}
\]

The $N^{th}$ partial sum is given by

\[
\sum_{n=1}^N \frac{1}{n^2 +n} = \frac{1}{2} + \frac{1}{6} + \frac{1}{12} + \cdots + \frac{1}{N^2 - N} + \frac{1}{N^2 + N}
\]
Note that the second to last term above comes from letting $n = N-1$, so that in the denominator we have 
\[
n^2 + n = (N-1)^2 + (N-1) = N^2 - 2N + 1 + N - 1 = N^2 -N.
\]
There does not appear to be an easy way to express this partial sum without simply listing all of the terms in the sum.
However, if we rewrite $\frac{1}{n^2 +n}$ using a partial fraction decomposition, we will see that the partial sum simplies greatly.
We have
\[
\frac{1}{n^2 + n} = \frac{1}{n(n+1)} = \frac{A}{n} + \frac{B}{n+1}.
\]
You can verify that $A = 1$ and $B=-1$, so that, in the end, we have
\[
\frac{1}{n^2 + n} = \frac{1}{n} - \frac{1}{n+1}.
\]
Using this form, we now rewrite the $N^{th}$ partial sum:
\[
\sum_{n=1}^N \frac{1}{n^2 +n} = \sum_{n=1}^N \left(\frac{1}{n}-\frac{1}{n+1}\right)
\]
\[
 = \left(\frac11 - \frac12 \right) + \left(\frac12 - \frac13 \right) + \left(\frac13 - \frac14 \right) + \cdots + 
 \left(\frac{1}{N-1} - \frac{1}{N} \right) +\left(\frac{1}{N} - \frac{1}{N+1} \right) 
\]
Looking carefully at the terms in this sum, we see lots of cancellation. For example, we see the terms $-\frac12$ and $+\frac12$.
We also see both $-\frac13$ and $+\frac13$ as well as both $-\frac{1}{N}$ and $+\frac{1}{N}$. In fact, every fraction will cancel out
except for the first and the last. The series collapses like an old-time telescope and the $N^{th}$ partial sum reduces to just
\[
S_N = \sum_{n=1}^N \frac{1}{n^2 +n} = 1 - \frac{1}{N+1}.
\]
Now, we can find the sum of the series by taking a limit:
\[
\sum_{n=1}^\infty  \frac{1}{n^2 +n} = \lim_{N\to \infty} \sum_{n=1}^N  \frac{1}{n^2 +n} = \lim_{N\to \infty} \left(1 - \frac{1}{N+1}\right) = 1-0 = 1.
\]
Thus, the series converges and its sum is 1.
\end{example}



\end{document}


\begin{example} %example #15
Find $h'(x)$ if $h(x) = x^{\sin(x)}$.\\
We will use the fact that the exponential and logarithm functions are inverses,
\[e^{\ln(x)} = x,\]
and the exponent property of logarithms, 
\[\ln(x^n) = n\ln(x),\]
to rewrite $h(x)$.  We have 
\[h(x) = x^{\sin(x)} = e^{\ln(x^{\sin(x)})} = e^{\sin(x)\ln(x)}\]
and we can now compute $h'(x)$ using a combination of the chain rule and product rule.
We can write $h(x)$ as a composition, $f(g(x))$ with 
\[g(x) = \sin(x)\ln(x) \quad \text{and} \quad f(x) = e^x.\]
Then to find $g'(x)$ we us the product rule and we get $g'(x) = \frac{\sin(x)}{x} + \cos(x)\ln(x)$.
Next $f'(x) = e^x$ and 
hence $f'(g(x)) = e^{g(x)} = e^{\sin(x)\ln(x)} = x^{\sin(x)}$.
We can then conclude $h'(x) = f'(g(x))g'(x) = x^{\sin(x)} \left[ \frac{\sin(x)}{x} + \cos(x)\ln(x)\right]$.
\end{example}

%more question formats below













%\begin{verbatim}
\begin{question}
What is your favorite color?
\begin{multipleChoice}
\choice[correct]{Rainbow}
\choice{Blue}
\choice{Green}
\choice{Red}
\end{multipleChoice}
\begin{freeResponse}
Hello
\end{freeResponse}
\end{question}
%\end{verbatim}





\begin{question}
  Which one will you choose?
  \begin{multipleChoice}
    \choice[correct]{I'm correct.}
    \choice{I'm wrong.}
    \choice{I'm wrong too.}
  \end{multipleChoice}
\end{question}


\begin{question}
  Which one will you choose?
  \begin{selectAll}
    \choice[correct]{I'm correct.}
    \choice{I'm wrong.}
    \choice[correct]{I'm also correct.}
    \choice{I'm wrong too.}
  \end{selectAll}
\end{question}


\begin{freeResponse}
What is the chain rule used for?
\end{freeResponse}
