\documentclass[handout]{ximera}

\input{../preamble}

\pgfplotsset{compat=1.13}

\outcome{Compute complex integrals}

\title{5.1 Contour Integrals}

\begin{document}

\begin{abstract}
We compute integrals of complex functions along contours.
\end{abstract}

\maketitle


Let $C$ be a contour parameterized by $\gamma(t) = x(t) + iy(t), \; a\leq t \leq b$ and let $f(z)$ be a complex function defined along $C$.
Then the integral of $f$ along $C$ is defined by
\[
\int_C f(z) dz = \int_a^b f(\gamma(t)) \gamma'(t) dt
\]

\begin{example}[example 1]
Compute $\dis \int_C \overline{z} dz$ where $C$ is the line segment from $-1$ to $1+i$.\\
We first parameterize the line segment. Since the equation of the line in the $xy$-plane is $y = \frac12x + \frac12$,
one possible parametrization of the line segment is
\[
\gamma(t) = x(t) + iy(t) = t + i\left(\frac{t}{2} + \frac12\right), \; -1 \leq t \leq 1
\]
The derivative of $\gamma(t)$ is 
\[
\gamma'(t) = 1 + \frac{i}{2}
\]
Next, $f(z) = \overline{z} = x-iy$ and hence
\[
f(\gamma(t)) = x(t) - iy(t) = t - i\left(\frac{t}{2} + \frac12\right)
\]
We are now ready to compute the contour integral:
\begin{align*}
\int_C \overline{z} \, dz &= \int_{-1}^1 \left[t - i\left(\frac{t}{2} + \frac12\right)\right]\cdot \left[1 + \frac{i}{2}\right] \, dt\\[6pt]
&= \int_{-1}^1 \left[t + \frac12\left(\frac{t}{2} + \frac12\right)\right] + i\left[-\left(\frac{t}{2} +\frac12\right) + \frac{t}{2}\right] \, dt\\[6pt]
&= \int_{-1}^1 \left[\frac54 t + \frac14\right]+i\left[-\frac12\right] \, dt\\[6pt]
&=\int_{-1}^1 \left[\frac54 t + \frac14\right] \, dt - i\int_{-1}^1  \frac12 \, dt\\[6pt]
                         &= \frac12 - i
\end{align*}
\end{example}

\begin{remark}
A line segment from $z_1$ to $z_2$ can be parameterized by $\gamma(t) = z_1 + t(z_2 - z_1), \, 0\leq t \leq 1$.
Since $(1+i) - (-1) = 2 + i$, the contour $C$ in the previous example can thus also be parametrized by
\[
\gamma(t) = -1 + t(2+i), \, 0 \leq t \leq 1
\]
\end{remark}

\begin{problem}(problem 1)
Use the parametrization given in the remark above to compute the integral in example 1.
\end{problem}

\begin{proposition}
If the contour $C$ has two different parametrizations, $\gamma_1(t) \, a_1 \leq t \leq b_1$ and $\gamma_2(t)\, a_2 \leq t \leq b_2$, then
\[
\int_C f(z) \, dz = \int_{a_1}^{b_1} f(\gamma_1(t)) \gamma_1'(t) \, dt = \int_{a_2}^{b_2} f(\gamma_2(t)) \gamma_2'(t) \, dt
\]
That is, the value of a contour integral is independent of the parametrization of the contour.
\end{proposition}

What happens if we reverse the direction of a contour , $C$?


If $C$ is a contour parameterized by $\gamma(t) = x(t) + iy(t), \, a \leq t \leq b$ then the contour $-C$ which represents the 
same points as $C$ but traced in the opposite 
direction has parametrization $\zeta(s) = x(a+b-s) + iy(a+b-s), \, a \leq s \leq b$.


\begin{proposition}
Suppose $f$ is continuous along a contour $C$ %parameterized by $C: \gamma(t) = x(t) + iy(t), \, a \leq t \leq b$
and suppose the contour $-C$ represents the same points as $C$ traced in the opposite direction, 
then 
\[
\int_{-C} f(z) \, dz = -\int_C f(z) \, dz
\]
\end{proposition}
\begin{proof}
Using the substitution $t = a+b-s$, we have
\begin{align*}
\int_{-C} f(z) \, dz &= \int_a^b f(\zeta(s)) \zeta'(s) \, ds \\
&= \int_a^b f\big(x(a+b-s) + iy(a+b-s)\big) \big[x'(a+b-s)(-1)+ iy'(a+b-s)(-1)\big]\, ds\\
                     &= \int_b^a f\big(x(t)+iy(t)\big) \big[x'(t)+ iy'(t)\big] \, dt\\
                     &= -\int_a^b f(\gamma(t)) \gamma'(t) \, dt\\
                   &= - \int_C f(z) \, dz
\end{align*}
\end{proof}

            
\end{document}


                         
                         



                         
















\begin{definition} 
A complex series  is defined as a limit of its sequence partial sums:
\[
\sum_{k=1}^\infty c_k = \lim_{n \to \infty}  \sum_{k=1}^n c_k = \lim_{n \to \infty} S_n
\]
If the sequence $\{S_n\}$ converges, then we say the series converges.  Otherwise, we say that the series diverges. 
\end{definition}

\begin{theorem}[Test for Divergence]
If $\dis \sum_{k=1}^\infty c_k$ converges, then $\dis \lim_{k\to\infty} c_k = 0$
\end{theorem}
\begin{proof}
Note that $c_n = S_n - S_{n-1}$, the difference in partial sums. Since the sequence $\{S_n\}$ converges, given $\epsilon >0$,
there exists a number $N$ and a number $S$ such that if $n>N$ then $|S_n - S| < \epsilon/2$. Hence for $n > N+1$, the triangle inequality gives
\begin{align*}
|c_n| &= |S_n - S_{n-1}| = |(S_n -S) + (S-S_{n-1})| \\
&\leq |S_n -S| + |S-S_{n-1}| < \frac{\epsilon}{2} + \frac{\epsilon}{2} =\epsilon
\end{align*}
Hence, the sequence $\{c_n\}$ converges to zero.
\end{proof}


\begin{example}[example 1] 
Determine whether the complex series $\dis \sum_{k=1}^\infty \frac{1+ik}{k}$ converges.\\
Since, $\dis \lim_{k \to \infty} \frac{1+ik}{k} = i$. Since $i \neq 0$, the Test for Divergence says that the series $\dis \sum_{k=1}^\infty \frac{1+ik}{k}$
does not converge, i.e., it diverges.
\end{example}

\begin{problem}(problem 1) 
Determine whether the complex series $\dis \sum_{k=0}^\infty \frac{k!}{(2i)^k}$ converges.\\
Since, $\dis \lim_{k \to \infty} \left|\frac{k!}{(2i)^k}\right| = \answer{\infty}$,\\
 $\dis \lim_{k \to \infty} \frac{k!}{(2i)^k} \neq \answer{0}$,\\
 the series $\dis \sum_{k=0}^\infty \frac{k!}{(2i)^k}\;\;$ \wordChoice{\choice{converges}\choice[correct]{diverges}}\\
 by the \wordChoice{\choice{Test for Convergence}\choice[correct]{Test for Divergence}}
\end{problem}

\begin{theorem}[Geometric Series]
Let $c \in \C$ and consider the series
\[
\sum_{k=0}^\infty c^k = 1 + c + c^2 + c^3 + \cdots
\]
This series converges if and only if $|c| < 1$.  Moreover, if it converges, its sum is 
$\displaystyle \frac{1}{1-c}$.
\end{theorem}

\begin{remark}
The complex number $c$ in the geometric series $\dis \sum_{k=0}^\infty c^k$ is called the common ratio of the series.
\end{remark}

\begin{proof}
Suppose $|c| < 1$. Then the partial sums have a closed form whose limit can be computed directly.
Since
\[
S_n = \sum_{k=1}^n c^k = 1+c+c^2+\cdots + c^n
\]
we have
\[
cS_n = c+c^2+\cdots + c^{n+1}
\]
Subtracting gives
\[
S_n - cS_n = 1-c^{n+1}
\]
from which we obtain the closed form
\[
S_n = \frac{1-c^{n+1}}{1-c}
\]
Now, since $|c|<1$, we have $c^n \to 0$ as $n \to \infty$ and hence
\[
\sum_{k=0}^\infty c^k = \lim_{n\to \infty} S_n = \lim_{n\to \infty} \frac{1-c^{n+1}}{1-c} = \frac{1}{1-c}
\]
Thus, the geometric series converges and its sum is also known.\\
If $|c| \geq 1$ then $c^n \nrightarrow 0$ as $n \to \infty$ which implies 
that the geometric series diverges (by the Test for Divergence).
\end{proof}


\begin{example}[example 2] 
Determine whether the geometric series converges or diverges:\\
a) $\;\;\dis \sum_{k=0}^\infty \frac{1}{(1+i)^k}\quad$  b) $\;\;\dis \sum_{k=0}^\infty \left(\frac{1+i}{1-i}\right)^k$ \\
Part a) This is a geometric series with common ratio $\dis \frac{1}{1+i}$. The modulus of the common ratio is 
\[
\left|\frac{1}{1+i}\right| = \frac{1}{\sqrt 2} <1
\]
Hence the geometric series converges and its sum is
\[
\sum_{k=0}^\infty \frac{1}{(1+i)^k} = \frac{1}{1-\frac{1}{1+i}} = \frac{1+i}{i} = 1-i
\]
Part b) This is a geometric series with common ratio $\dis \frac{1+i}{1-i}$. The modulus of the common ratio is 
\[
\left|\frac{1+i}{1-i}\right| = \frac{\sqrt 2}{\sqrt 2} = 1 \nless 1
\]
Hence the geometric series diverges.
\end{example}


\begin{problem}(problem 2)
Determine whether the geometric series converges or diverges. If it converges, find its sum: $\;\;\dis \sum_{k=0}^\infty \left(\frac{2i}{2+i}\right)$ \\
The common ratio is $\; \answer{\frac{2i}{2+i}}$\\
The modulus of the common ratio is $\; \answer{\frac{2}{\sqrt 5}}$\\
Is this less than 1? \wordChoice{\choice[correct]{yes}\choice{no}}\\
The geometric series  \wordChoice{\choice[correct]{converges}\choice{diverges}}\\
The sum of the series is $\; \answer{\frac{2+i}{2-i}}$
\end{problem}


\begin{theorem}[Absolute Convergence]
If the series $\dis \sum_{k=1}^\infty |c_k|$ converges, then so does the complex series $\dis \sum_{k=1}^\infty c_k$.
\end{theorem}


\begin{remark}
To prove this result, we will need the Monotone Convergence Theorem which states that a bounded, monotone sequence of real numbers converges.
\end{remark}

\begin{proof}
Suppose $\displaystyle \sum_{k=1}^\infty |c_k|$ converges to the real number $S$, and break the partial sums of  the complex series 
$\displaystyle \sum_{k=1}^\infty c_k$ into their real and imaginary parts:
\[
\sum_{k=1}^n c_k =  \sum_{k=1}^n a_k + i\sum_{k=1}^n b_k
\]
where $a_k, b_k \in \R$ for all $k$.  Let $a_k^+ = a_k$ if $a_k \geq 0$ and let $a_k^+ = 0$ if $a_k < 0$.
Similarly, let $a_k^- = -a_k$ if $a_k < 0$ and let $a_k^- = 0$ if $a_k \geq 0$. Then 
\[
\sum_{k=1}^n a_k = \sum_{k=1}^n a_k^+ - \sum_{k=1}^n a_k^- = A_n^+ - A_n^-
\]
The sequences $\{A_n^+\}$ and $\{A_n^-\}$ are both increasing sequences and since $|a_k| \leq |c_k|$ for all $k$, they are both bounded above by $S$.
Hence, by the Monotone Convergence Theorem, both sequences converge.
Thus, the real series $\dis \sum_{k=1}^n a_k$ converges, to a sum, $A$. Applying the same argument to the partial sums of the imaginary part, 
$\dis \sum_{k=1}^n b_k$, we see that it too converges to a sum, $B$. Finally, we can conclude that $\dis \sum_{k=1}^\infty c_k$ converges to $A + iB$. 
\end{proof}

\begin{example}[example 3]
Show that the complex series converges: $\dis \sum_{k=1}^\infty \frac{2e^i}{(k+ik)^2}$\\
The modulus of $c_k$ is
\[
\left|\frac{2e^i}{(k+ik)^2}\right| = \frac{2}{2k^2} = \frac{1}{k^2}
\]
and the series
\[
\sum_{k=1}^\infty \frac{1}{k^2}
\]
is a convergent $p$-series with $p = 2 > 1$. Moreover the sum of this well known series is $\frac{\pi^2}{6}$.
\end{example}

\begin{problem}(problem 3) 
Determine whether the complex series $\dis \sum_{k=0}^\infty \frac{i^k}{k!}$ converges.\\
The modulus of $c_k$ is $\; \answer{1/k!}$\\
The series $\dis \sum_{k=0}^\infty \frac{1}{k!}\;\;$ \wordChoice{\choice[correct]{converges}\choice{diverges}}\\
The series $\dis \sum_{k=0}^\infty \frac{i^k}{k!}\;\;$ \wordChoice{\choice[correct]{converges}\choice{diverges}}
\end{problem}


\begin{definition}
We define the limit superior of a sequence of real numbers $\{a_n\}, \; \limsup_{n \to \infty} a_n,\;$to be the largest limit of any subsequence of $\{a_n\}$.\
\end{definition}


\begin{remark}
If the sequence $\{a_n\}$ converges to $a$, then $\limsup_{n \to \infty} a_n =a$.
\end{remark}

\begin{remark}
It is possible that $\limsup_{n \to \infty} a_n =\pm\infty$
\end{remark}

\begin{example}[example 4]
Find the limit superior of the sequence $\{c_k\}= \{1, 2, 3, 1, 2, 3, 1, 2, 3, \ldots\}$
The sequence $\{c_k\}$ has subsequences that converge to $1, 2$ and $3$. Since the largest of these limits is $3$, we have
\[
\limsup_{k\to\infty} c_k = 3
\]
\end{example}

\begin{problem}(problem 4)
Find the limit superior of the sequence:\\
a) $\dis\; \{(-1)^k\} \quad \limsup_{k\to\infty} (-1)^k = \; \answer{1}$\\
a) $\dis\; \{c_k\} = \{1, -1, \frac12, -1, \frac13, -1, \ldots\} \quad \limsup_{k\to\infty} c_k = \; \answer{0}$\\
\end{problem}


\begin{theorem}[Root Test]
Let $\displaystyle \sum_{k=1}^\infty c_k$ be a complex series and let 
\[
L = \limsup_{k \to \infty} \sqrt[k]{|c_k|}
\]
Then the series converges if $L <1$ and diverges if $L >1$.
\end{theorem}

\begin{proof}
First, suppose $\dis L = \limsup_{k \to \infty} \sqrt[k]{|c_k|} < 1$. Then there exists a natural number $N$ such that for $k>N 
|c_k| < L^k$.  Hence the series $\dis \sum_{k = N+1}^\infty |c_k|$ converges by direct comparison to the geometric series
$\dis \sum_{k = N+1}^\infty L^k$. Thus, the series $\dis\sum_{k = 1}^\infty c_k$ converges absolutely and is therefore convergent.\\
Next, suppose $\dis L = \limsup_{k \to \infty} \sqrt[k]{|c_k|} > 1$ Then there exists a subsequence of $\{c_k\}$ such that $\sqrt[k]{|c_k|} > 1$
which implies that $|c_k| > 1$ for each of the infinitely many terms in this subsequence. Hence, $c_k \nrightarrow 0$ as $k \to \infty$.
By the Test for Divergence, the series $\displaystyle \sum_{k=1}^\infty c_k$ diverges.
\end{proof}

\begin{remark}
The series $\dis \sum_{k=1}^\infty \frac{1}{k^2}$ and $\dis \sum_{k=1}^\infty \frac{1}{k}$ show that if $L = 1$ in the Root Test,
then no conclusion can be drawn. This is because the first series converges and the second series diverges but $L=1$ in both cases.
\end{remark}

\begin{example}[example 5]
Determine if the series converges or diverges: $\dis \sum_{k=1}^\infty \left(\frac{k+i}{k^2 - i}\right)^k$\\
Computing the $k^{th}$ root of the modulus of $c_k$ gives
\[
\sqrt[k]{|c_k|} = \sqrt[k]{\left|\left(\frac{k+i}{k^2 - i}\right)^k\right|} = \sqrt[k]{\left|\frac{k+i}{k^2 - i}\right|^k} = \sqrt{\frac{k^2 + 1}{k^4 + 1}}
\]
and the limit superior is
\[
\limsup_{k \to \infty} \sqrt[k]{|c_k|} = \limsup_{k \to \infty}  \sqrt{\frac{k^2 + 1}{k^4 + 1}} = 0 <1
\]
so the series converges.
\end{example}


\begin{problem}(problem 5)
Determine if the series converges or diverges: 
\[
\sum_{k=1}^\infty \left(\frac{e^{ik}}{1+i\sqrt k}\right)^k
\]
$\sqrt[k]{|c_k|} = \; \answer{\frac{1}{\sqrt{1+k}}}$\\
The limit superior is $\; \limsup_{k\to\infty}\sqrt[k]{|c_k|}= \; \answer{0}$\\
Is this less than 1? \wordChoice{\choice[correct]{yes}\choice{no}}\\
The series  \wordChoice{\choice[correct]{converges}\choice{diverges}}
\end{problem}

\begin{theorem}[Ratio Test]
Let $\displaystyle \sum_{k=1}^\infty c_k$ be a complex series and let 
\[
L = \limsup_{k \to \infty} \left|\frac{c_{k+1}}{c_k}\right|
\]
Then the series converges if $L <1$ and diverges if $L >1$.
\end{theorem}

\begin{remark} 
If $c_k = 0$ for infinitely many values of $k$, then the ratio test cannot be used.
\end{remark}
\begin{remark} 
The proof of the ratio test is similar to the proof of the root test.
\end{remark}

\begin{example}[example 6]
Determine if the series converges or diverges: 
\[
\sum_{k=0}^\infty \frac{i^k2^k}{k!}
\]
The modulus of the ratio of successive terms is
\[
\left|\frac{i^{k+1}2^{k+1}}{(k+1)!}\cdot \frac{k!}{i^k 2^k}\right| = \frac{2}{k+1}
\]
Taking the limit gives
\[
\limsup_{k \to \infty} \frac{2}{k+1} = 0 < 1
\]
By the Ratio Test, the series converges.
\end{example}

\begin{problem}(problem 6)
Determine if the series converges or diverges: 
\[
\sum_{k=0}^\infty \frac{2e^{ik}}{(2k)!}
\]
$\left|\frac{c_{k+1}}{c_k}\right| = \; \answer{\frac{1}{(k+1)(2k+1)}}$\\
The limit superior is $\; \limsup_{k\to\infty}\left|\frac{c_{k+1}}{c_k}\right|= \; \answer{0}$\\
Is this less than 1? \wordChoice{\choice[correct]{yes}\choice{no}}\\
The series  \wordChoice{\choice[correct]{converges}\choice{diverges}}
\end{problem}


\end{document}




